Renamed some lemmas with better names.

src/Corecursive_Prop.thy
@@ -25,7 +25,7 @@ fun TESL_interpretation_atomic_stepwise
 where
   \<open>\<lbrakk> K\<^sub>1 sporadic \<tau> on K\<^sub>2 \<rbrakk>\<^sub>T\<^sub>E\<^sub>S\<^sub>L\<^bsup>\<ge> i\<^esup> =
       {\<rho>. \<exists>n\<ge>i. ticks ((Rep_run \<rho>) n K\<^sub>1) \<and> time ((Rep_run \<rho>) n K\<^sub>2) = \<tau>}\<close>
-| \<open>\<lbrakk> K\<^sub>1 sporadic-add \<lparr>\<tau>\<^sub>v\<^sub>a\<^sub>r(K\<^sub>p\<^sub>a\<^sub>s\<^sub>t, n\<^sub>p\<^sub>a\<^sub>s\<^sub>t) \<oplus> \<delta>\<tau>\<rparr> on K\<^sub>2 \<rbrakk>\<^sub>T\<^sub>E\<^sub>S\<^sub>L\<^bsup>\<ge> i\<^esup> =
+| \<open>\<lbrakk> K\<^sub>1 sporadic\<sharp> \<lparr>\<tau>\<^sub>v\<^sub>a\<^sub>r(K\<^sub>p\<^sub>a\<^sub>s\<^sub>t, n\<^sub>p\<^sub>a\<^sub>s\<^sub>t) \<oplus> \<delta>\<tau>\<rparr> on K\<^sub>2 \<rbrakk>\<^sub>T\<^sub>E\<^sub>S\<^sub>L\<^bsup>\<ge> i\<^esup> =
       {\<rho>. \<exists>n\<ge>i. ticks ((Rep_run \<rho>) n K\<^sub>1)
                          \<and> time ((Rep_run \<rho>) n K\<^sub>2) = time ((Rep_run \<rho>) n\<^sub>p\<^sub>a\<^sub>s\<^sub>t K\<^sub>p\<^sub>a\<^sub>s\<^sub>t) + \<delta>\<tau> }\<close>
 | \<open>\<lbrakk> time-relation \<lfloor>K\<^sub>1, K\<^sub>2\<rfloor> \<in> R \<rbrakk>\<^sub>T\<^sub>E\<^sub>S\<^sub>L\<^bsup>\<ge> i\<^esup> =
@@ -41,7 +41,7 @@ where
                          \<longrightarrow> ticks ((Rep_run \<rho>) m slave)
                )
       }\<close>
-| \<open>\<lbrakk> master time-delayed2 by \<delta>\<tau> on measuring implies slave \<rbrakk>\<^sub>T\<^sub>E\<^sub>S\<^sub>L\<^bsup>\<ge> i\<^esup> =
+| \<open>\<lbrakk> master time-delayed\<sharp> by \<delta>\<tau> on measuring implies slave \<rbrakk>\<^sub>T\<^sub>E\<^sub>S\<^sub>L\<^bsup>\<ge> i\<^esup> =
       {\<rho>. \<forall>n\<ge>i. ticks ((Rep_run \<rho>) n master) \<longrightarrow>
                (let measured_time = time ((Rep_run \<rho>) n measuring) in
                 \<exists>m \<ge> n. ticks ((Rep_run \<rho>) m slave)
@@ -63,8 +63,8 @@ lemma TESL_interp_unfold_stepwise_sporadicon:
   \<open>\<lbrakk> K\<^sub>1 sporadic \<tau> on K\<^sub>2 \<rbrakk>\<^sub>T\<^sub>E\<^sub>S\<^sub>L = \<Union> {Y. \<exists>n::nat. Y = \<lbrakk> K\<^sub>1 sporadic \<tau> on K\<^sub>2 \<rbrakk>\<^sub>T\<^sub>E\<^sub>S\<^sub>L\<^bsup>\<ge> n\<^esup>}\<close>
 by auto
 
-lemma TESL_interp_unfold_stepwise_sporadicon_add:
-  \<open>\<lbrakk> K\<^sub>1 sporadic-add \<tau>\<^sub>e\<^sub>x\<^sub>p\<^sub>r on K\<^sub>2 \<rbrakk>\<^sub>T\<^sub>E\<^sub>S\<^sub>L = \<Union> {Y. \<exists>n::nat. Y = \<lbrakk> K\<^sub>1 sporadic-add \<tau>\<^sub>e\<^sub>x\<^sub>p\<^sub>r on K\<^sub>2 \<rbrakk>\<^sub>T\<^sub>E\<^sub>S\<^sub>L\<^bsup>\<ge> n\<^esup>}\<close>
+lemma TESL_interp_unfold_stepwise_sporadicon_tvar:
+  \<open>\<lbrakk> K\<^sub>1 sporadic\<sharp> \<tau>\<^sub>e\<^sub>x\<^sub>p\<^sub>r on K\<^sub>2 \<rbrakk>\<^sub>T\<^sub>E\<^sub>S\<^sub>L = \<Union> {Y. \<exists>n::nat. Y = \<lbrakk> K\<^sub>1 sporadic\<sharp> \<tau>\<^sub>e\<^sub>x\<^sub>p\<^sub>r on K\<^sub>2 \<rbrakk>\<^sub>T\<^sub>E\<^sub>S\<^sub>L\<^bsup>\<ge> n\<^esup>}\<close>
 proof (induction \<tau>\<^sub>e\<^sub>x\<^sub>p\<^sub>r)
   case (AddDelay x1a \<tau>)
   then show ?case 
@@ -99,10 +99,10 @@ lemma TESL_interp_unfold_stepwise_timedelayed:
           Y = \<lbrakk> master time-delayed by \<delta>\<tau> on measuring implies slave \<rbrakk>\<^sub>T\<^sub>E\<^sub>S\<^sub>L\<^bsup>\<ge> n\<^esup>}\<close>
 by auto
 
-lemma TESL_interp_unfold_stepwise_timedelayed2:
-  \<open>\<lbrakk> master time-delayed2 by \<delta>\<tau> on measuring implies slave \<rbrakk>\<^sub>T\<^sub>E\<^sub>S\<^sub>L
+lemma TESL_interp_unfold_stepwise_timedelayed_tvar:
+  \<open>\<lbrakk> master time-delayed\<sharp> by \<delta>\<tau> on measuring implies slave \<rbrakk>\<^sub>T\<^sub>E\<^sub>S\<^sub>L
     = \<Inter> {Y. \<exists>n::nat.
-          Y = \<lbrakk> master time-delayed2 by \<delta>\<tau> on measuring implies slave \<rbrakk>\<^sub>T\<^sub>E\<^sub>S\<^sub>L\<^bsup>\<ge> n\<^esup>}\<close>
+          Y = \<lbrakk> master time-delayed\<sharp> by \<delta>\<tau> on measuring implies slave \<rbrakk>\<^sub>T\<^sub>E\<^sub>S\<^sub>L\<^bsup>\<ge> n\<^esup>}\<close>
 by auto
 
 lemma TESL_interp_unfold_stepwise_weakly_precedes:
@@ -131,7 +131,7 @@ theorem TESL_interp_unfold_stepwise_positive_atoms:
 proof (cases \<phi>)
   case SporadicOn thus ?thesis using TESL_interp_unfold_stepwise_sporadicon by simp
 next
-  case SporadicAdd thus ?thesis using TESL_interp_unfold_stepwise_sporadicon_add by simp
+  case SporadicOnTvar thus ?thesis using TESL_interp_unfold_stepwise_sporadicon_tvar by simp
 next
   case TagRelation thus ?thesis using assms by simp
 next
@@ -141,7 +141,7 @@ next
 next
   case TimeDelayedBy thus ?thesis using assms by simp
 next
-  case TimeDelayedBy2 thus ?thesis using assms by simp
+  case TimeDelayedByTvar thus ?thesis using assms by simp
 next
   case WeaklyPrecedes thus ?thesis using assms by simp
 next
@@ -168,7 +168,7 @@ theorem TESL_interp_unfold_stepwise_negative_atoms:
 proof (cases \<phi>)
   case SporadicOn thus ?thesis using assms by simp
 next
-  case SporadicAdd thus ?thesis using assms by simp
+  case SporadicOnTvar thus ?thesis using assms by simp
 next
   case TagRelation
     thus ?thesis using TESL_interp_unfold_stepwise_tagrelgen by simp
@@ -182,8 +182,8 @@ next
   case TimeDelayedBy
     thus ?thesis using TESL_interp_unfold_stepwise_timedelayed by simp
 next
-  case TimeDelayedBy2
-    thus ?thesis using TESL_interp_unfold_stepwise_timedelayed2 by simp
+  case TimeDelayedByTvar
+    thus ?thesis using TESL_interp_unfold_stepwise_timedelayed_tvar by simp
 next
   case WeaklyPrecedes
     thus ?thesis
@@ -266,10 +266,10 @@ using exists_nat_set_suc[of \<open>n\<close> \<open>\<lambda>\<rho> n. ticks (Re
                                      \<and> time (Rep_run \<rho> n K\<^sub>2) = \<tau>\<close>]
 by (simp add: Collect_conj_eq)
 
-lemma TESL_interp_stepwise_sporadicon_add_coind_unfold:
-  \<open>\<lbrakk> K\<^sub>1 sporadic-add \<lparr>\<tau>\<^sub>v\<^sub>a\<^sub>r(K, n') \<oplus> \<tau>\<rparr> on K\<^sub>2 \<rbrakk>\<^sub>T\<^sub>E\<^sub>S\<^sub>L\<^bsup>\<ge> n\<^esup> =
-    \<lbrakk> K\<^sub>1 \<Up> n \<rbrakk>\<^sub>p\<^sub>r\<^sub>i\<^sub>m \<inter> \<lbrakk> K\<^sub>2 \<Down> n @@ \<lparr>\<tau>\<^sub>v\<^sub>a\<^sub>r(K, n') \<oplus> \<tau>\<rparr> \<rbrakk>\<^sub>p\<^sub>r\<^sub>i\<^sub>m
-    \<union> \<lbrakk> K\<^sub>1 sporadic-add \<lparr>\<tau>\<^sub>v\<^sub>a\<^sub>r(K, n') \<oplus> \<tau>\<rparr> on K\<^sub>2 \<rbrakk>\<^sub>T\<^sub>E\<^sub>S\<^sub>L\<^bsup>\<ge> Suc n\<^esup>\<close>
+lemma TESL_interp_stepwise_sporadicon_tvar_coind_unfold:
+  \<open>\<lbrakk> K\<^sub>1 sporadic\<sharp> \<lparr>\<tau>\<^sub>v\<^sub>a\<^sub>r(K, n') \<oplus> \<tau>\<rparr> on K\<^sub>2 \<rbrakk>\<^sub>T\<^sub>E\<^sub>S\<^sub>L\<^bsup>\<ge> n\<^esup> =
+    \<lbrakk> K\<^sub>1 \<Up> n \<rbrakk>\<^sub>p\<^sub>r\<^sub>i\<^sub>m \<inter> \<lbrakk> K\<^sub>2 \<Down> n @\<sharp> \<lparr>\<tau>\<^sub>v\<^sub>a\<^sub>r(K, n') \<oplus> \<tau>\<rparr> \<rbrakk>\<^sub>p\<^sub>r\<^sub>i\<^sub>m
+    \<union> \<lbrakk> K\<^sub>1 sporadic\<sharp> \<lparr>\<tau>\<^sub>v\<^sub>a\<^sub>r(K, n') \<oplus> \<tau>\<rparr> on K\<^sub>2 \<rbrakk>\<^sub>T\<^sub>E\<^sub>S\<^sub>L\<^bsup>\<ge> Suc n\<^esup>\<close>
 proof -
   have "{ \<rho>. \<exists>m\<ge>n. ticks ((Rep_run \<rho>) m K\<^sub>1) = True \<and> time ((Rep_run \<rho>) m K\<^sub>2) = time ((Rep_run \<rho>) n' K) + \<tau> }
       = { \<rho>. ticks ((Rep_run \<rho>) n K\<^sub>1) = True \<and> time ((Rep_run \<rho>) n K\<^sub>2) = time ((Rep_run \<rho>) n' K) + \<tau>
@@ -278,12 +278,12 @@ proof -
   then show ?thesis by auto
 qed
 
-lemma TESL_interp_stepwise_sporadicon_add_coind_unfold2:
-  \<open>\<lbrakk> K\<^sub>1 sporadic-add \<tau>\<^sub>e\<^sub>x\<^sub>p\<^sub>r on K\<^sub>2 \<rbrakk>\<^sub>T\<^sub>E\<^sub>S\<^sub>L\<^bsup>\<ge> n\<^esup> =
-    \<lbrakk> K\<^sub>1 \<Up> n \<rbrakk>\<^sub>p\<^sub>r\<^sub>i\<^sub>m \<inter> \<lbrakk> K\<^sub>2 \<Down> n @@ \<tau>\<^sub>e\<^sub>x\<^sub>p\<^sub>r \<rbrakk>\<^sub>p\<^sub>r\<^sub>i\<^sub>m        \<comment> \<open>rule @{term sporadic_add_e2}\<close>
-    \<union> \<lbrakk> K\<^sub>1 sporadic-add \<tau>\<^sub>e\<^sub>x\<^sub>p\<^sub>r on K\<^sub>2 \<rbrakk>\<^sub>T\<^sub>E\<^sub>S\<^sub>L\<^bsup>\<ge> Suc n\<^esup>\<close>   \<comment> \<open>rule @{term sporadic_add_e1}\<close>
-using TESL_interp_stepwise_sporadicon_add_coind_unfold
-by (metis old.prod.exhaust tag_expr.exhaust tag_val.exhaust)
+lemma TESL_interp_stepwise_sporadicon_tvar_coind_unfold2:
+  \<open>\<lbrakk> K\<^sub>1 sporadic\<sharp> \<tau>\<^sub>e\<^sub>x\<^sub>p\<^sub>r on K\<^sub>2 \<rbrakk>\<^sub>T\<^sub>E\<^sub>S\<^sub>L\<^bsup>\<ge> n\<^esup> =
+    \<lbrakk> K\<^sub>1 \<Up> n \<rbrakk>\<^sub>p\<^sub>r\<^sub>i\<^sub>m \<inter> \<lbrakk> K\<^sub>2 \<Down> n @\<sharp> \<tau>\<^sub>e\<^sub>x\<^sub>p\<^sub>r \<rbrakk>\<^sub>p\<^sub>r\<^sub>i\<^sub>m        \<comment> \<open>rule @{term sporadic_on_tvar_e2}\<close>
+    \<union> \<lbrakk> K\<^sub>1 sporadic\<sharp> \<tau>\<^sub>e\<^sub>x\<^sub>p\<^sub>r on K\<^sub>2 \<rbrakk>\<^sub>T\<^sub>E\<^sub>S\<^sub>L\<^bsup>\<ge> Suc n\<^esup>\<close>   \<comment> \<open>rule @{term sporadic_on_tvar_e1}\<close>
+using TESL_interp_stepwise_sporadicon_tvar_coind_unfold
+by (metis old.prod.exhaust tag_expr.exhaust tag_var.exhaust)
 
 lemma TESL_interp_stepwise_tagrel_coind_unfold:
   \<open>\<lbrakk> time-relation \<lfloor>K\<^sub>1, K\<^sub>2\<rfloor> \<in> R \<rbrakk>\<^sub>T\<^sub>E\<^sub>S\<^sub>L\<^bsup>\<ge> n\<^esup> =        \<comment> \<open>rule @{term tagrel_e}\<close>
@@ -365,12 +365,12 @@ next
   } thus "{x. P x n} \<inter> {x. \<forall>m \<ge> Suc n. P x m} \<subseteq> {x. \<forall>m \<ge> n. P x m}" ..
 qed
 
-lemma TESL_interp_stepwise_timedelayed2_coind_unfold:
-  \<open>\<lbrakk> master time-delayed2 by \<delta>\<tau> on measuring implies slave \<rbrakk>\<^sub>T\<^sub>E\<^sub>S\<^sub>L\<^bsup>\<ge> n\<^esup> =
-     (     \<lbrakk> master \<not>\<Up> n \<rbrakk>\<^sub>p\<^sub>r\<^sub>i\<^sub>m               \<comment> \<open>rule @{term timedelayed2_e1}\<close>
-        \<union> (\<lbrakk> master \<Up> n \<rbrakk>\<^sub>p\<^sub>r\<^sub>i\<^sub>m \<inter> \<lbrakk> slave sporadic-add \<lparr>\<tau>\<^sub>v\<^sub>a\<^sub>r(measuring, n) \<oplus> \<delta>\<tau>\<rparr> on measuring \<rbrakk>\<^sub>T\<^sub>E\<^sub>S\<^sub>L\<^bsup>\<ge> n\<^esup>))
-                                             \<comment> \<open>rule @{term timedelayed2_e2}\<close>
-     \<inter> \<lbrakk> master time-delayed2 by \<delta>\<tau> on measuring implies slave \<rbrakk>\<^sub>T\<^sub>E\<^sub>S\<^sub>L\<^bsup>\<ge> Suc n\<^esup>\<close>
+lemma TESL_interp_stepwise_timedelayed_tvar_coind_unfold:
+  \<open>\<lbrakk> master time-delayed\<sharp> by \<delta>\<tau> on measuring implies slave \<rbrakk>\<^sub>T\<^sub>E\<^sub>S\<^sub>L\<^bsup>\<ge> n\<^esup> =
+     (     \<lbrakk> master \<not>\<Up> n \<rbrakk>\<^sub>p\<^sub>r\<^sub>i\<^sub>m               \<comment> \<open>rule @{term timedelayed_tvar_e1}\<close>
+        \<union> (\<lbrakk> master \<Up> n \<rbrakk>\<^sub>p\<^sub>r\<^sub>i\<^sub>m \<inter> \<lbrakk> slave sporadic\<sharp> \<lparr>\<tau>\<^sub>v\<^sub>a\<^sub>r(measuring, n) \<oplus> \<delta>\<tau>\<rparr> on measuring \<rbrakk>\<^sub>T\<^sub>E\<^sub>S\<^sub>L\<^bsup>\<ge> n\<^esup>))
+                                             \<comment> \<open>rule @{term timedelayed_tvar_e2}\<close>
+     \<inter> \<lbrakk> master time-delayed\<sharp> by \<delta>\<tau> on measuring implies slave \<rbrakk>\<^sub>T\<^sub>E\<^sub>S\<^sub>L\<^bsup>\<ge> Suc n\<^esup>\<close>
 proof -
   have "{ \<rho>. \<forall>m\<ge>n. ticks ((Rep_run \<rho>) m master) \<longrightarrow>
                (let measured_time = time ((Rep_run \<rho>) m measuring) in
@@ -488,7 +488,7 @@ proof (induction \<phi>)
 case (SporadicOn x1 x2 x3)
   then show ?case by simp
 next
-  case (SporadicAdd K\<^sub>1 \<tau>\<^sub>e\<^sub>x\<^sub>p\<^sub>r K\<^sub>2)
+  case (SporadicOnTvar K\<^sub>1 \<tau>\<^sub>e\<^sub>x\<^sub>p\<^sub>r K\<^sub>2)
   then show ?case 
   proof (induction \<tau>\<^sub>e\<^sub>x\<^sub>p\<^sub>r)
     case (AddDelay \<tau>\<^sub>v\<^sub>a\<^sub>r\<^sub>0 \<delta>\<tau>)
@@ -515,7 +515,7 @@ next
   case (TimeDelayedBy x1 x2 x3 x4)
 then show ?case by simp
 next
-  case (TimeDelayedBy2 x1 x2 x3 x4)
+  case (TimeDelayedByTvar x1 x2 x3 x4)
   then show ?case by simp
 next
   case (WeaklyPrecedes x1 x2)
@@ -549,12 +549,12 @@ text \<open>
   \<^item> the interpretation of its present from the current instant,
   \<^item> the interpretation of its future from the next instant.
 \<close>
-fun HeronConf_interpretation
+fun configuration_interpretation
   ::\<open>'\<tau>::linordered_field config \<Rightarrow> '\<tau> run set\<close>          (\<open>\<lbrakk> _ \<rbrakk>\<^sub>c\<^sub>o\<^sub>n\<^sub>f\<^sub>i\<^sub>g\<close> 71)
 where
   \<open>\<lbrakk> \<Gamma>, n \<turnstile> \<Psi> \<triangleright> \<Phi> \<rbrakk>\<^sub>c\<^sub>o\<^sub>n\<^sub>f\<^sub>i\<^sub>g = \<lbrakk>\<lbrakk> \<Gamma> \<rbrakk>\<rbrakk>\<^sub>p\<^sub>r\<^sub>i\<^sub>m \<inter> \<lbrakk>\<lbrakk> \<Psi> \<rbrakk>\<rbrakk>\<^sub>T\<^sub>E\<^sub>S\<^sub>L\<^bsup>\<ge> n\<^esup> \<inter> \<lbrakk>\<lbrakk> \<Phi> \<rbrakk>\<rbrakk>\<^sub>T\<^sub>E\<^sub>S\<^sub>L\<^bsup>\<ge> Suc n\<^esup>\<close>
 
-lemma HeronConf_interp_composition:
+lemma configuration_interp_composition:
    \<open>\<lbrakk> \<Gamma>\<^sub>1, n \<turnstile> \<Psi>\<^sub>1 \<triangleright> \<Phi>\<^sub>1 \<rbrakk>\<^sub>c\<^sub>o\<^sub>n\<^sub>f\<^sub>i\<^sub>g \<inter> \<lbrakk> \<Gamma>\<^sub>2, n \<turnstile> \<Psi>\<^sub>2 \<triangleright> \<Phi>\<^sub>2 \<rbrakk>\<^sub>c\<^sub>o\<^sub>n\<^sub>f\<^sub>i\<^sub>g
      = \<lbrakk> (\<Gamma>\<^sub>1 @ \<Gamma>\<^sub>2), n \<turnstile> (\<Psi>\<^sub>1 @ \<Psi>\<^sub>2) \<triangleright> (\<Phi>\<^sub>1 @ \<Phi>\<^sub>2) \<rbrakk>\<^sub>c\<^sub>o\<^sub>n\<^sub>f\<^sub>i\<^sub>g\<close>
   using TESL_interp_stepwise_composition symrun_interp_expansion
@@ -566,7 +566,7 @@ text \<open>
   a configuration is the same as the configuration at the next instant of its future.
   This corresponds to the introduction rule of the operational semantics.
 \<close>
-lemma HeronConf_interp_stepwise_instant_cases:
+lemma configuration_interp_stepwise_instant_cases:
    \<open>\<lbrakk> \<Gamma>, n \<turnstile> [] \<triangleright> \<Phi> \<rbrakk>\<^sub>c\<^sub>o\<^sub>n\<^sub>f\<^sub>i\<^sub>g = \<lbrakk> \<Gamma>, Suc n \<turnstile> \<Phi> \<triangleright> [] \<rbrakk>\<^sub>c\<^sub>o\<^sub>n\<^sub>f\<^sub>i\<^sub>g\<close>
 proof -
   have \<open>\<lbrakk> \<Gamma>, n \<turnstile> [] \<triangleright> \<Phi> \<rbrakk>\<^sub>c\<^sub>o\<^sub>n\<^sub>f\<^sub>i\<^sub>g = \<lbrakk>\<lbrakk> \<Gamma> \<rbrakk>\<rbrakk>\<^sub>p\<^sub>r\<^sub>i\<^sub>m \<inter> \<lbrakk>\<lbrakk> [] \<rbrakk>\<rbrakk>\<^sub>T\<^sub>E\<^sub>S\<^sub>L\<^bsup>\<ge> n\<^esup> \<inter> \<lbrakk>\<lbrakk> \<Phi> \<rbrakk>\<rbrakk>\<^sub>T\<^sub>E\<^sub>S\<^sub>L\<^bsup>\<ge> Suc n\<^esup>\<close>
@@ -585,7 +585,7 @@ text \<open>
   semantics to give rewriting rules for the interpretation of configurations that
   match the elimination rules of the operational semantics.
 \<close>
-lemma HeronConf_interp_stepwise_sporadicon_cases:
+lemma configuration_interp_stepwise_sporadicon_cases:
    \<open>\<lbrakk> \<Gamma>, n \<turnstile> ((K\<^sub>1 sporadic \<tau> on K\<^sub>2) # \<Psi>) \<triangleright> \<Phi> \<rbrakk>\<^sub>c\<^sub>o\<^sub>n\<^sub>f\<^sub>i\<^sub>g
     = \<lbrakk> \<Gamma>, n \<turnstile> \<Psi> \<triangleright> ((K\<^sub>1 sporadic \<tau> on K\<^sub>2) # \<Phi>) \<rbrakk>\<^sub>c\<^sub>o\<^sub>n\<^sub>f\<^sub>i\<^sub>g
     \<union> \<lbrakk> ((K\<^sub>1 \<Up> n) # (K\<^sub>2 \<Down> n @ \<tau>) # \<Gamma>), n \<turnstile> \<Psi> \<triangleright> \<Phi> \<rbrakk>\<^sub>c\<^sub>o\<^sub>n\<^sub>f\<^sub>i\<^sub>g\<close>
@@ -614,10 +614,10 @@ proof -
   qed
 qed
 
-lemma HeronConf_interp_stepwise_sporadicon_add_cases:
-   \<open>\<lbrakk> \<Gamma>, n \<turnstile> ((K\<^sub>1 sporadic-add \<tau>\<^sub>e\<^sub>x\<^sub>p\<^sub>r on K\<^sub>2) # \<Psi>) \<triangleright> \<Phi> \<rbrakk>\<^sub>c\<^sub>o\<^sub>n\<^sub>f\<^sub>i\<^sub>g
-    = \<lbrakk> \<Gamma>, n \<turnstile> \<Psi> \<triangleright> ((K\<^sub>1 sporadic-add \<tau>\<^sub>e\<^sub>x\<^sub>p\<^sub>r on K\<^sub>2) # \<Phi>) \<rbrakk>\<^sub>c\<^sub>o\<^sub>n\<^sub>f\<^sub>i\<^sub>g
-    \<union> \<lbrakk> ((K\<^sub>1 \<Up> n) # (K\<^sub>2 \<Down> n @@ \<tau>\<^sub>e\<^sub>x\<^sub>p\<^sub>r) # \<Gamma>), n \<turnstile> \<Psi> \<triangleright> \<Phi> \<rbrakk>\<^sub>c\<^sub>o\<^sub>n\<^sub>f\<^sub>i\<^sub>g\<close>
+lemma configuration_interp_stepwise_sporadicon_tvar_cases:
+   \<open>\<lbrakk> \<Gamma>, n \<turnstile> ((K\<^sub>1 sporadic\<sharp> \<tau>\<^sub>e\<^sub>x\<^sub>p\<^sub>r on K\<^sub>2) # \<Psi>) \<triangleright> \<Phi> \<rbrakk>\<^sub>c\<^sub>o\<^sub>n\<^sub>f\<^sub>i\<^sub>g
+    = \<lbrakk> \<Gamma>, n \<turnstile> \<Psi> \<triangleright> ((K\<^sub>1 sporadic\<sharp> \<tau>\<^sub>e\<^sub>x\<^sub>p\<^sub>r on K\<^sub>2) # \<Phi>) \<rbrakk>\<^sub>c\<^sub>o\<^sub>n\<^sub>f\<^sub>i\<^sub>g
+    \<union> \<lbrakk> ((K\<^sub>1 \<Up> n) # (K\<^sub>2 \<Down> n @\<sharp> \<tau>\<^sub>e\<^sub>x\<^sub>p\<^sub>r) # \<Gamma>), n \<turnstile> \<Psi> \<triangleright> \<Phi> \<rbrakk>\<^sub>c\<^sub>o\<^sub>n\<^sub>f\<^sub>i\<^sub>g\<close>
 proof (induction \<tau>\<^sub>e\<^sub>x\<^sub>p\<^sub>r)
   case (AddDelay x1a \<delta>\<tau>)
   then show ?case
@@ -628,11 +628,11 @@ proof (induction \<tau>\<^sub>e\<^sub>x\<^sub>p\<^sub>r)
         case (Pair K\<^sub>p\<^sub>a\<^sub>s\<^sub>t n\<^sub>p\<^sub>a\<^sub>s\<^sub>t)
         then show ?case
         proof -
-          have "(\<lbrakk> K\<^sub>1 \<Up> n \<rbrakk>\<^sub>p\<^sub>r\<^sub>i\<^sub>m \<inter> \<lbrakk> K\<^sub>2 \<Down> n @@ \<lparr> \<tau>\<^sub>v\<^sub>a\<^sub>r (K\<^sub>p\<^sub>a\<^sub>s\<^sub>t, n\<^sub>p\<^sub>a\<^sub>s\<^sub>t) \<oplus> \<delta>\<tau> \<rparr> \<rbrakk>\<^sub>p\<^sub>r\<^sub>i\<^sub>m \<union> \<lbrakk> K\<^sub>1 sporadic-add \<lparr> \<tau>\<^sub>v\<^sub>a\<^sub>r (K\<^sub>p\<^sub>a\<^sub>s\<^sub>t, n\<^sub>p\<^sub>a\<^sub>s\<^sub>t) \<oplus> \<delta>\<tau> \<rparr> on K\<^sub>2 \<rbrakk>\<^sub>T\<^sub>E\<^sub>S\<^sub>L\<^bsup>\<ge> Suc n\<^esup>) \<inter> (\<lbrakk>\<lbrakk> \<Gamma> \<rbrakk>\<rbrakk>\<^sub>p\<^sub>r\<^sub>i\<^sub>m \<inter> \<lbrakk>\<lbrakk> \<Psi> \<rbrakk>\<rbrakk>\<^sub>T\<^sub>E\<^sub>S\<^sub>L\<^bsup>\<ge> n\<^esup>) = \<lbrakk> K\<^sub>1 sporadic-add \<lparr> \<tau>\<^sub>v\<^sub>a\<^sub>r (K\<^sub>p\<^sub>a\<^sub>s\<^sub>t, n\<^sub>p\<^sub>a\<^sub>s\<^sub>t) \<oplus> \<delta>\<tau> \<rparr> on K\<^sub>2 \<rbrakk>\<^sub>T\<^sub>E\<^sub>S\<^sub>L\<^bsup>\<ge> n\<^esup> \<inter> (\<lbrakk>\<lbrakk> \<Psi> \<rbrakk>\<rbrakk>\<^sub>T\<^sub>E\<^sub>S\<^sub>L\<^bsup>\<ge> n\<^esup> \<inter> \<lbrakk>\<lbrakk> \<Gamma> \<rbrakk>\<rbrakk>\<^sub>p\<^sub>r\<^sub>i\<^sub>m)"
-            by (metis Int_commute TESL_interp_stepwise_sporadicon_add_coind_unfold)
-          then have "\<lbrakk>\<lbrakk> K\<^sub>1 \<Up> n # K\<^sub>2 \<Down> n @@ \<lparr> \<tau>\<^sub>v\<^sub>a\<^sub>r (K\<^sub>p\<^sub>a\<^sub>s\<^sub>t, n\<^sub>p\<^sub>a\<^sub>s\<^sub>t) \<oplus> \<delta>\<tau> \<rparr> # \<Gamma> \<rbrakk>\<rbrakk>\<^sub>p\<^sub>r\<^sub>i\<^sub>m \<inter> \<lbrakk>\<lbrakk> \<Psi> \<rbrakk>\<rbrakk>\<^sub>T\<^sub>E\<^sub>S\<^sub>L\<^bsup>\<ge> n\<^esup> \<union> \<lbrakk>\<lbrakk> \<Gamma> \<rbrakk>\<rbrakk>\<^sub>p\<^sub>r\<^sub>i\<^sub>m \<inter> \<lbrakk>\<lbrakk> \<Psi> \<rbrakk>\<rbrakk>\<^sub>T\<^sub>E\<^sub>S\<^sub>L\<^bsup>\<ge> n\<^esup> \<inter> \<lbrakk> K\<^sub>1 sporadic-add \<lparr> \<tau>\<^sub>v\<^sub>a\<^sub>r (K\<^sub>p\<^sub>a\<^sub>s\<^sub>t, n\<^sub>p\<^sub>a\<^sub>s\<^sub>t) \<oplus> \<delta>\<tau> \<rparr> on K\<^sub>2 \<rbrakk>\<^sub>T\<^sub>E\<^sub>S\<^sub>L\<^bsup>\<ge> Suc n\<^esup> = \<lbrakk>\<lbrakk> \<Gamma> \<rbrakk>\<rbrakk>\<^sub>p\<^sub>r\<^sub>i\<^sub>m \<inter> \<lbrakk>\<lbrakk> (K\<^sub>1 sporadic-add \<lparr> \<tau>\<^sub>v\<^sub>a\<^sub>r (K\<^sub>p\<^sub>a\<^sub>s\<^sub>t, n\<^sub>p\<^sub>a\<^sub>s\<^sub>t) \<oplus> \<delta>\<tau> \<rparr> on K\<^sub>2) # \<Psi> \<rbrakk>\<rbrakk>\<^sub>T\<^sub>E\<^sub>S\<^sub>L\<^bsup>\<ge> n\<^esup>"
+          have "(\<lbrakk> K\<^sub>1 \<Up> n \<rbrakk>\<^sub>p\<^sub>r\<^sub>i\<^sub>m \<inter> \<lbrakk> K\<^sub>2 \<Down> n @\<sharp> \<lparr> \<tau>\<^sub>v\<^sub>a\<^sub>r (K\<^sub>p\<^sub>a\<^sub>s\<^sub>t, n\<^sub>p\<^sub>a\<^sub>s\<^sub>t) \<oplus> \<delta>\<tau> \<rparr> \<rbrakk>\<^sub>p\<^sub>r\<^sub>i\<^sub>m \<union> \<lbrakk> K\<^sub>1 sporadic\<sharp> \<lparr> \<tau>\<^sub>v\<^sub>a\<^sub>r (K\<^sub>p\<^sub>a\<^sub>s\<^sub>t, n\<^sub>p\<^sub>a\<^sub>s\<^sub>t) \<oplus> \<delta>\<tau> \<rparr> on K\<^sub>2 \<rbrakk>\<^sub>T\<^sub>E\<^sub>S\<^sub>L\<^bsup>\<ge> Suc n\<^esup>) \<inter> (\<lbrakk>\<lbrakk> \<Gamma> \<rbrakk>\<rbrakk>\<^sub>p\<^sub>r\<^sub>i\<^sub>m \<inter> \<lbrakk>\<lbrakk> \<Psi> \<rbrakk>\<rbrakk>\<^sub>T\<^sub>E\<^sub>S\<^sub>L\<^bsup>\<ge> n\<^esup>) = \<lbrakk> K\<^sub>1 sporadic\<sharp> \<lparr> \<tau>\<^sub>v\<^sub>a\<^sub>r (K\<^sub>p\<^sub>a\<^sub>s\<^sub>t, n\<^sub>p\<^sub>a\<^sub>s\<^sub>t) \<oplus> \<delta>\<tau> \<rparr> on K\<^sub>2 \<rbrakk>\<^sub>T\<^sub>E\<^sub>S\<^sub>L\<^bsup>\<ge> n\<^esup> \<inter> (\<lbrakk>\<lbrakk> \<Psi> \<rbrakk>\<rbrakk>\<^sub>T\<^sub>E\<^sub>S\<^sub>L\<^bsup>\<ge> n\<^esup> \<inter> \<lbrakk>\<lbrakk> \<Gamma> \<rbrakk>\<rbrakk>\<^sub>p\<^sub>r\<^sub>i\<^sub>m)"
+            by (metis Int_commute TESL_interp_stepwise_sporadicon_tvar_coind_unfold)
+          then have "\<lbrakk>\<lbrakk> K\<^sub>1 \<Up> n # K\<^sub>2 \<Down> n @\<sharp> \<lparr> \<tau>\<^sub>v\<^sub>a\<^sub>r (K\<^sub>p\<^sub>a\<^sub>s\<^sub>t, n\<^sub>p\<^sub>a\<^sub>s\<^sub>t) \<oplus> \<delta>\<tau> \<rparr> # \<Gamma> \<rbrakk>\<rbrakk>\<^sub>p\<^sub>r\<^sub>i\<^sub>m \<inter> \<lbrakk>\<lbrakk> \<Psi> \<rbrakk>\<rbrakk>\<^sub>T\<^sub>E\<^sub>S\<^sub>L\<^bsup>\<ge> n\<^esup> \<union> \<lbrakk>\<lbrakk> \<Gamma> \<rbrakk>\<rbrakk>\<^sub>p\<^sub>r\<^sub>i\<^sub>m \<inter> \<lbrakk>\<lbrakk> \<Psi> \<rbrakk>\<rbrakk>\<^sub>T\<^sub>E\<^sub>S\<^sub>L\<^bsup>\<ge> n\<^esup> \<inter> \<lbrakk> K\<^sub>1 sporadic\<sharp> \<lparr> \<tau>\<^sub>v\<^sub>a\<^sub>r (K\<^sub>p\<^sub>a\<^sub>s\<^sub>t, n\<^sub>p\<^sub>a\<^sub>s\<^sub>t) \<oplus> \<delta>\<tau> \<rparr> on K\<^sub>2 \<rbrakk>\<^sub>T\<^sub>E\<^sub>S\<^sub>L\<^bsup>\<ge> Suc n\<^esup> = \<lbrakk>\<lbrakk> \<Gamma> \<rbrakk>\<rbrakk>\<^sub>p\<^sub>r\<^sub>i\<^sub>m \<inter> \<lbrakk>\<lbrakk> (K\<^sub>1 sporadic\<sharp> \<lparr> \<tau>\<^sub>v\<^sub>a\<^sub>r (K\<^sub>p\<^sub>a\<^sub>s\<^sub>t, n\<^sub>p\<^sub>a\<^sub>s\<^sub>t) \<oplus> \<delta>\<tau> \<rparr> on K\<^sub>2) # \<Psi> \<rbrakk>\<rbrakk>\<^sub>T\<^sub>E\<^sub>S\<^sub>L\<^bsup>\<ge> n\<^esup>"
             by auto
-          then have "\<lbrakk> \<Gamma>, n \<turnstile> (K\<^sub>1 sporadic-add \<lparr> \<tau>\<^sub>v\<^sub>a\<^sub>r (K\<^sub>p\<^sub>a\<^sub>s\<^sub>t, n\<^sub>p\<^sub>a\<^sub>s\<^sub>t) \<oplus> \<delta>\<tau> \<rparr> on K\<^sub>2) # \<Psi> \<triangleright> \<Phi> \<rbrakk>\<^sub>c\<^sub>o\<^sub>n\<^sub>f\<^sub>i\<^sub>g = \<lbrakk> K\<^sub>1 \<Up> n # K\<^sub>2 \<Down> n @@ \<lparr> \<tau>\<^sub>v\<^sub>a\<^sub>r (K\<^sub>p\<^sub>a\<^sub>s\<^sub>t, n\<^sub>p\<^sub>a\<^sub>s\<^sub>t) \<oplus> \<delta>\<tau> \<rparr> # \<Gamma>, n \<turnstile> \<Psi> \<triangleright> \<Phi> \<rbrakk>\<^sub>c\<^sub>o\<^sub>n\<^sub>f\<^sub>i\<^sub>g \<union> \<lbrakk> \<Gamma>, n \<turnstile> \<Psi> \<triangleright> (K\<^sub>1 sporadic-add \<lparr> \<tau>\<^sub>v\<^sub>a\<^sub>r (K\<^sub>p\<^sub>a\<^sub>s\<^sub>t, n\<^sub>p\<^sub>a\<^sub>s\<^sub>t) \<oplus> \<delta>\<tau> \<rparr> on K\<^sub>2) # \<Phi> \<rbrakk>\<^sub>c\<^sub>o\<^sub>n\<^sub>f\<^sub>i\<^sub>g"
+          then have "\<lbrakk> \<Gamma>, n \<turnstile> (K\<^sub>1 sporadic\<sharp> \<lparr> \<tau>\<^sub>v\<^sub>a\<^sub>r (K\<^sub>p\<^sub>a\<^sub>s\<^sub>t, n\<^sub>p\<^sub>a\<^sub>s\<^sub>t) \<oplus> \<delta>\<tau> \<rparr> on K\<^sub>2) # \<Psi> \<triangleright> \<Phi> \<rbrakk>\<^sub>c\<^sub>o\<^sub>n\<^sub>f\<^sub>i\<^sub>g = \<lbrakk> K\<^sub>1 \<Up> n # K\<^sub>2 \<Down> n @\<sharp> \<lparr> \<tau>\<^sub>v\<^sub>a\<^sub>r (K\<^sub>p\<^sub>a\<^sub>s\<^sub>t, n\<^sub>p\<^sub>a\<^sub>s\<^sub>t) \<oplus> \<delta>\<tau> \<rparr> # \<Gamma>, n \<turnstile> \<Psi> \<triangleright> \<Phi> \<rbrakk>\<^sub>c\<^sub>o\<^sub>n\<^sub>f\<^sub>i\<^sub>g \<union> \<lbrakk> \<Gamma>, n \<turnstile> \<Psi> \<triangleright> (K\<^sub>1 sporadic\<sharp> \<lparr> \<tau>\<^sub>v\<^sub>a\<^sub>r (K\<^sub>p\<^sub>a\<^sub>s\<^sub>t, n\<^sub>p\<^sub>a\<^sub>s\<^sub>t) \<oplus> \<delta>\<tau> \<rparr> on K\<^sub>2) # \<Phi> \<rbrakk>\<^sub>c\<^sub>o\<^sub>n\<^sub>f\<^sub>i\<^sub>g"
             by auto
           then show ?thesis
             by blast
@@ -641,7 +641,7 @@ proof (induction \<tau>\<^sub>e\<^sub>x\<^sub>p\<^sub>r)
   qed
 qed
 
-lemma HeronConf_interp_stepwise_tagrel_cases:
+lemma configuration_interp_stepwise_tagrel_cases:
    \<open>\<lbrakk> \<Gamma>, n \<turnstile> ((time-relation \<lfloor>K\<^sub>1, K\<^sub>2\<rfloor> \<in> R) # \<Psi>) \<triangleright> \<Phi> \<rbrakk>\<^sub>c\<^sub>o\<^sub>n\<^sub>f\<^sub>i\<^sub>g
     = \<lbrakk> ((\<lfloor>\<tau>\<^sub>v\<^sub>a\<^sub>r(K\<^sub>1, n), \<tau>\<^sub>v\<^sub>a\<^sub>r(K\<^sub>2, n)\<rfloor> \<in> R) # \<Gamma>), n
         \<turnstile> \<Psi> \<triangleright> ((time-relation \<lfloor>K\<^sub>1, K\<^sub>2\<rfloor> \<in> R) # \<Phi>) \<rbrakk>\<^sub>c\<^sub>o\<^sub>n\<^sub>f\<^sub>i\<^sub>g\<close>
@@ -665,7 +665,7 @@ proof -
   qed
 qed
 
-lemma HeronConf_interp_stepwise_implies_cases:
+lemma configuration_interp_stepwise_implies_cases:
    \<open>\<lbrakk> \<Gamma>, n \<turnstile> ((K\<^sub>1 implies K\<^sub>2) # \<Psi>) \<triangleright> \<Phi> \<rbrakk>\<^sub>c\<^sub>o\<^sub>n\<^sub>f\<^sub>i\<^sub>g
       = \<lbrakk> ((K\<^sub>1 \<not>\<Up> n) # \<Gamma>), n \<turnstile> \<Psi> \<triangleright> ((K\<^sub>1 implies K\<^sub>2) # \<Phi>) \<rbrakk>\<^sub>c\<^sub>o\<^sub>n\<^sub>f\<^sub>i\<^sub>g
       \<union> \<lbrakk> ((K\<^sub>1 \<Up> n) # (K\<^sub>2 \<Up> n) # \<Gamma>), n \<turnstile> \<Psi> \<triangleright> ((K\<^sub>1 implies K\<^sub>2) # \<Phi>) \<rbrakk>\<^sub>c\<^sub>o\<^sub>n\<^sub>f\<^sub>i\<^sub>g\<close>
@@ -698,7 +698,7 @@ proof -
   qed
 qed
 
-lemma HeronConf_interp_stepwise_implies_not_cases:
+lemma configuration_interp_stepwise_implies_not_cases:
    \<open>\<lbrakk> \<Gamma>, n \<turnstile> ((K\<^sub>1 implies not K\<^sub>2) # \<Psi>) \<triangleright> \<Phi> \<rbrakk>\<^sub>c\<^sub>o\<^sub>n\<^sub>f\<^sub>i\<^sub>g
       = \<lbrakk> ((K\<^sub>1 \<not>\<Up> n) # \<Gamma>), n \<turnstile> \<Psi> \<triangleright> ((K\<^sub>1 implies not K\<^sub>2) # \<Phi>) \<rbrakk>\<^sub>c\<^sub>o\<^sub>n\<^sub>f\<^sub>i\<^sub>g
       \<union> \<lbrakk> ((K\<^sub>1 \<Up> n) # (K\<^sub>2 \<not>\<Up> n) # \<Gamma>), n \<turnstile> \<Psi> \<triangleright> ((K\<^sub>1 implies not K\<^sub>2) # \<Phi>) \<rbrakk>\<^sub>c\<^sub>o\<^sub>n\<^sub>f\<^sub>i\<^sub>g\<close>
@@ -732,7 +732,7 @@ proof -
   qed
 qed
 
-lemma HeronConf_interp_stepwise_timedelayed_cases:
+lemma configuration_interp_stepwise_timedelayed_cases:
   \<open>\<lbrakk> \<Gamma>, n \<turnstile> ((K\<^sub>1 time-delayed by \<delta>\<tau> on K\<^sub>2 implies K\<^sub>3) # \<Psi>) \<triangleright> \<Phi> \<rbrakk>\<^sub>c\<^sub>o\<^sub>n\<^sub>f\<^sub>i\<^sub>g
     = \<lbrakk> ((K\<^sub>1 \<not>\<Up> n) # \<Gamma>), n \<turnstile> \<Psi> \<triangleright> ((K\<^sub>1 time-delayed by \<delta>\<tau> on K\<^sub>2 implies K\<^sub>3) # \<Phi>) \<rbrakk>\<^sub>c\<^sub>o\<^sub>n\<^sub>f\<^sub>i\<^sub>g
     \<union> \<lbrakk> ((K\<^sub>1 \<Up> n) # (K\<^sub>2 @ n \<oplus> \<delta>\<tau> \<Rightarrow> K\<^sub>3) # \<Gamma>), n
@@ -776,21 +776,21 @@ proof -
   qed
 qed
 
-lemma HeronConf_interp_stepwise_timedelayed2_cases:
-  \<open>\<lbrakk> \<Gamma>, n \<turnstile> ((K\<^sub>1 time-delayed2 by \<delta>\<tau> on K\<^sub>2 implies K\<^sub>3) # \<Psi>) \<triangleright> \<Phi> \<rbrakk>\<^sub>c\<^sub>o\<^sub>n\<^sub>f\<^sub>i\<^sub>g
-    = \<lbrakk> ((K\<^sub>1 \<not>\<Up> n) # \<Gamma>), n \<turnstile> \<Psi> \<triangleright> ((K\<^sub>1 time-delayed2 by \<delta>\<tau> on K\<^sub>2 implies K\<^sub>3) # \<Phi>) \<rbrakk>\<^sub>c\<^sub>o\<^sub>n\<^sub>f\<^sub>i\<^sub>g
+lemma configuration_interp_stepwise_timedelayed_tvar_cases:
+  \<open>\<lbrakk> \<Gamma>, n \<turnstile> ((K\<^sub>1 time-delayed\<sharp> by \<delta>\<tau> on K\<^sub>2 implies K\<^sub>3) # \<Psi>) \<triangleright> \<Phi> \<rbrakk>\<^sub>c\<^sub>o\<^sub>n\<^sub>f\<^sub>i\<^sub>g
+    = \<lbrakk> ((K\<^sub>1 \<not>\<Up> n) # \<Gamma>), n \<turnstile> \<Psi> \<triangleright> ((K\<^sub>1 time-delayed\<sharp> by \<delta>\<tau> on K\<^sub>2 implies K\<^sub>3) # \<Phi>) \<rbrakk>\<^sub>c\<^sub>o\<^sub>n\<^sub>f\<^sub>i\<^sub>g
     \<union> \<lbrakk> ((K\<^sub>1 \<Up> n) # \<Gamma>), n
-        \<turnstile> (K\<^sub>3 sporadic-add \<lparr>\<tau>\<^sub>v\<^sub>a\<^sub>r(K\<^sub>2, n) \<oplus> \<delta>\<tau>\<rparr> on K\<^sub>2) # \<Psi> \<triangleright> ((K\<^sub>1 time-delayed2 by \<delta>\<tau> on K\<^sub>2 implies K\<^sub>3) # \<Phi>) \<rbrakk>\<^sub>c\<^sub>o\<^sub>n\<^sub>f\<^sub>i\<^sub>g\<close>
+        \<turnstile> (K\<^sub>3 sporadic\<sharp> \<lparr>\<tau>\<^sub>v\<^sub>a\<^sub>r(K\<^sub>2, n) \<oplus> \<delta>\<tau>\<rparr> on K\<^sub>2) # \<Psi> \<triangleright> ((K\<^sub>1 time-delayed\<sharp> by \<delta>\<tau> on K\<^sub>2 implies K\<^sub>3) # \<Phi>) \<rbrakk>\<^sub>c\<^sub>o\<^sub>n\<^sub>f\<^sub>i\<^sub>g\<close>
 proof -
-  have "\<lbrakk>\<lbrakk> \<Psi> \<rbrakk>\<rbrakk>\<^sub>T\<^sub>E\<^sub>S\<^sub>L\<^bsup>\<ge> n\<^esup> \<inter> (\<lbrakk> K\<^sub>1 \<not>\<Up> n \<rbrakk>\<^sub>p\<^sub>r\<^sub>i\<^sub>m \<union> \<lbrakk> K\<^sub>1 \<Up> n \<rbrakk>\<^sub>p\<^sub>r\<^sub>i\<^sub>m \<inter> \<lbrakk> K\<^sub>3 sporadic-add \<lparr> \<tau>\<^sub>v\<^sub>a\<^sub>r (K\<^sub>2, n) \<oplus> \<delta>\<tau> \<rparr> on K\<^sub>2 \<rbrakk>\<^sub>T\<^sub>E\<^sub>S\<^sub>L\<^bsup>\<ge> n\<^esup>) \<inter> \<lbrakk> K\<^sub>1 time-delayed2 by \<delta>\<tau> on K\<^sub>2 implies K\<^sub>3 \<rbrakk>\<^sub>T\<^sub>E\<^sub>S\<^sub>L\<^bsup>\<ge> Suc n\<^esup> = \<lbrakk>\<lbrakk> \<Psi> \<rbrakk>\<rbrakk>\<^sub>T\<^sub>E\<^sub>S\<^sub>L\<^bsup>\<ge> n\<^esup> \<inter> \<lbrakk> K\<^sub>1 time-delayed2 by \<delta>\<tau> on K\<^sub>2 implies K\<^sub>3 \<rbrakk>\<^sub>T\<^sub>E\<^sub>S\<^sub>L\<^bsup>\<ge> n\<^esup>"
-    by (metis Int_assoc TESL_interp_stepwise_timedelayed2_coind_unfold)
-  then have "\<lbrakk> \<Gamma>, n \<turnstile> (K\<^sub>1 time-delayed2 by \<delta>\<tau> on K\<^sub>2 implies K\<^sub>3) # \<Psi> \<triangleright> \<Phi> \<rbrakk>\<^sub>c\<^sub>o\<^sub>n\<^sub>f\<^sub>i\<^sub>g = \<lbrakk>\<lbrakk> \<Psi> \<rbrakk>\<rbrakk>\<^sub>T\<^sub>E\<^sub>S\<^sub>L\<^bsup>\<ge> n\<^esup> \<inter> (\<lbrakk> K\<^sub>1 \<not>\<Up> n \<rbrakk>\<^sub>p\<^sub>r\<^sub>i\<^sub>m \<union> \<lbrakk> K\<^sub>1 \<Up> n \<rbrakk>\<^sub>p\<^sub>r\<^sub>i\<^sub>m \<inter> \<lbrakk> K\<^sub>3 sporadic-add \<lparr> \<tau>\<^sub>v\<^sub>a\<^sub>r (K\<^sub>2, n) \<oplus> \<delta>\<tau> \<rparr> on K\<^sub>2 \<rbrakk>\<^sub>T\<^sub>E\<^sub>S\<^sub>L\<^bsup>\<ge> n\<^esup>) \<inter> \<lbrakk> K\<^sub>1 time-delayed2 by \<delta>\<tau> on K\<^sub>2 implies K\<^sub>3 \<rbrakk>\<^sub>T\<^sub>E\<^sub>S\<^sub>L\<^bsup>\<ge> Suc n\<^esup> \<inter> (\<lbrakk>\<lbrakk> \<Phi> \<rbrakk>\<rbrakk>\<^sub>T\<^sub>E\<^sub>S\<^sub>L\<^bsup>\<ge> Suc n\<^esup> \<inter> \<lbrakk>\<lbrakk> \<Gamma> \<rbrakk>\<rbrakk>\<^sub>p\<^sub>r\<^sub>i\<^sub>m)"
+  have "\<lbrakk>\<lbrakk> \<Psi> \<rbrakk>\<rbrakk>\<^sub>T\<^sub>E\<^sub>S\<^sub>L\<^bsup>\<ge> n\<^esup> \<inter> (\<lbrakk> K\<^sub>1 \<not>\<Up> n \<rbrakk>\<^sub>p\<^sub>r\<^sub>i\<^sub>m \<union> \<lbrakk> K\<^sub>1 \<Up> n \<rbrakk>\<^sub>p\<^sub>r\<^sub>i\<^sub>m \<inter> \<lbrakk> K\<^sub>3 sporadic\<sharp> \<lparr> \<tau>\<^sub>v\<^sub>a\<^sub>r (K\<^sub>2, n) \<oplus> \<delta>\<tau> \<rparr> on K\<^sub>2 \<rbrakk>\<^sub>T\<^sub>E\<^sub>S\<^sub>L\<^bsup>\<ge> n\<^esup>) \<inter> \<lbrakk> K\<^sub>1 time-delayed\<sharp> by \<delta>\<tau> on K\<^sub>2 implies K\<^sub>3 \<rbrakk>\<^sub>T\<^sub>E\<^sub>S\<^sub>L\<^bsup>\<ge> Suc n\<^esup> = \<lbrakk>\<lbrakk> \<Psi> \<rbrakk>\<rbrakk>\<^sub>T\<^sub>E\<^sub>S\<^sub>L\<^bsup>\<ge> n\<^esup> \<inter> \<lbrakk> K\<^sub>1 time-delayed\<sharp> by \<delta>\<tau> on K\<^sub>2 implies K\<^sub>3 \<rbrakk>\<^sub>T\<^sub>E\<^sub>S\<^sub>L\<^bsup>\<ge> n\<^esup>"
+    by (metis Int_assoc TESL_interp_stepwise_timedelayed_tvar_coind_unfold)
+  then have "\<lbrakk> \<Gamma>, n \<turnstile> (K\<^sub>1 time-delayed\<sharp> by \<delta>\<tau> on K\<^sub>2 implies K\<^sub>3) # \<Psi> \<triangleright> \<Phi> \<rbrakk>\<^sub>c\<^sub>o\<^sub>n\<^sub>f\<^sub>i\<^sub>g = \<lbrakk>\<lbrakk> \<Psi> \<rbrakk>\<rbrakk>\<^sub>T\<^sub>E\<^sub>S\<^sub>L\<^bsup>\<ge> n\<^esup> \<inter> (\<lbrakk> K\<^sub>1 \<not>\<Up> n \<rbrakk>\<^sub>p\<^sub>r\<^sub>i\<^sub>m \<union> \<lbrakk> K\<^sub>1 \<Up> n \<rbrakk>\<^sub>p\<^sub>r\<^sub>i\<^sub>m \<inter> \<lbrakk> K\<^sub>3 sporadic\<sharp> \<lparr> \<tau>\<^sub>v\<^sub>a\<^sub>r (K\<^sub>2, n) \<oplus> \<delta>\<tau> \<rparr> on K\<^sub>2 \<rbrakk>\<^sub>T\<^sub>E\<^sub>S\<^sub>L\<^bsup>\<ge> n\<^esup>) \<inter> \<lbrakk> K\<^sub>1 time-delayed\<sharp> by \<delta>\<tau> on K\<^sub>2 implies K\<^sub>3 \<rbrakk>\<^sub>T\<^sub>E\<^sub>S\<^sub>L\<^bsup>\<ge> Suc n\<^esup> \<inter> (\<lbrakk>\<lbrakk> \<Phi> \<rbrakk>\<rbrakk>\<^sub>T\<^sub>E\<^sub>S\<^sub>L\<^bsup>\<ge> Suc n\<^esup> \<inter> \<lbrakk>\<lbrakk> \<Gamma> \<rbrakk>\<rbrakk>\<^sub>p\<^sub>r\<^sub>i\<^sub>m)"
     by force
   then show ?thesis
     by auto
 qed
 
-lemma HeronConf_interp_stepwise_weakly_precedes_cases:
+lemma configuration_interp_stepwise_weakly_precedes_cases:
    \<open>\<lbrakk> \<Gamma>, n \<turnstile> ((K\<^sub>1 weakly precedes K\<^sub>2) # \<Psi>) \<triangleright> \<Phi> \<rbrakk>\<^sub>c\<^sub>o\<^sub>n\<^sub>f\<^sub>i\<^sub>g
     = \<lbrakk> ((\<lceil>#\<^sup>\<le> K\<^sub>2 n, #\<^sup>\<le> K\<^sub>1 n\<rceil> \<in> (\<lambda>(x,y). x\<le>y)) # \<Gamma>), n
       \<turnstile> \<Psi> \<triangleright> ((K\<^sub>1 weakly precedes K\<^sub>2) # \<Phi>) \<rbrakk>\<^sub>c\<^sub>o\<^sub>n\<^sub>f\<^sub>i\<^sub>g\<close>
@@ -814,7 +814,7 @@ proof -
   qed
 qed
 
-lemma HeronConf_interp_stepwise_strictly_precedes_cases:
+lemma configuration_interp_stepwise_strictly_precedes_cases:
    \<open>\<lbrakk> \<Gamma>, n \<turnstile> ((K\<^sub>1 strictly precedes K\<^sub>2) # \<Psi>) \<triangleright> \<Phi> \<rbrakk>\<^sub>c\<^sub>o\<^sub>n\<^sub>f\<^sub>i\<^sub>g
     = \<lbrakk> ((\<lceil>#\<^sup>\<le> K\<^sub>2 n, #\<^sup>< K\<^sub>1 n\<rceil> \<in> (\<lambda>(x,y). x\<le>y)) # \<Gamma>), n
       \<turnstile> \<Psi> \<triangleright> ((K\<^sub>1 strictly precedes K\<^sub>2) # \<Phi>) \<rbrakk>\<^sub>c\<^sub>o\<^sub>n\<^sub>f\<^sub>i\<^sub>g\<close>
@@ -838,7 +838,7 @@ proof -
   qed
 qed
 
-lemma HeronConf_interp_stepwise_kills_cases:
+lemma configuration_interp_stepwise_kills_cases:
    \<open>\<lbrakk> \<Gamma>, n \<turnstile> ((K\<^sub>1 kills K\<^sub>2) # \<Psi>) \<triangleright> \<Phi> \<rbrakk>\<^sub>c\<^sub>o\<^sub>n\<^sub>f\<^sub>i\<^sub>g
     = \<lbrakk> ((K\<^sub>1 \<not>\<Up> n) # \<Gamma>), n \<turnstile> \<Psi> \<triangleright> ((K\<^sub>1 kills K\<^sub>2) # \<Phi>) \<rbrakk>\<^sub>c\<^sub>o\<^sub>n\<^sub>f\<^sub>i\<^sub>g
     \<union> \<lbrakk> ((K\<^sub>1 \<Up> n) # (K\<^sub>2 \<not>\<Up> \<ge> n) # \<Gamma>), n \<turnstile> \<Psi> \<triangleright> ((K\<^sub>1 kills K\<^sub>2) # \<Phi>) \<rbrakk>\<^sub>c\<^sub>o\<^sub>n\<^sub>f\<^sub>i\<^sub>g\<close>
