src/TESL.thy
@@ -25,33 +25,31 @@ datatype     '\<tau> tag_const =  TConst   (the_tag_const : '\<tau>)         (\<
 text\<open>
   Tag values are used to refer to the time on a clock at a given instant index.
 \<close>
-datatype tag_val =
+(* TODO: text *)
+datatype tag_var =
   TSchematic \<open>clock * instant_index\<close> (\<open>\<tau>\<^sub>v\<^sub>a\<^sub>r\<close>)
 datatype '\<tau> tag_expr      =  (* Const    "'\<tau> tag_const"          ("\<lparr> _ \<rparr>") *)
-                              AddDelay "tag_val" "'\<tau> tag_const" ("\<lparr> _ \<oplus> _ \<rparr>")
-(* datatype tag_var          =  TSchematic "clock * instant_index" ("\<tau>\<^sub>v\<^sub>a\<^sub>r")
-datatype '\<tau> tag_expr      =  Const    "'\<tau> tag_const"          ("\<lparr> _ \<rparr>")
-                           |  AddDelay "tag_var" "'\<tau> tag_const" ("\<lparr> _ \<oplus> _ \<rparr>") *)
+                              AddDelay "tag_var" "'\<tau> tag_const" ("\<lparr> _ \<oplus> _ \<rparr>")
 
 subsection\<open>Operators for the TESL language\<close>
 text\<open>
   The type of atomic TESL constraints, which can be combined to form specifications.
 \<close>
 datatype '\<tau> TESL_atomic =
-    SporadicOn       \<open>clock\<close> \<open>'\<tau> tag_const\<close>  \<open>clock\<close>  (\<open>_ sporadic _ on _\<close> 55)
-  | SporadicAdd      \<open>clock\<close> \<open>'\<tau> tag_expr\<close>  \<open>clock\<close>   (\<open>_ sporadic-add _ on _\<close> 55) 
-  | TagRelation      \<open>clock\<close> \<open>clock\<close> \<open>('\<tau> tag_const \<times> '\<tau> tag_const) \<Rightarrow> bool\<close> 
+    SporadicOn         \<open>clock\<close> \<open>'\<tau> tag_const\<close>  \<open>clock\<close>  (\<open>_ sporadic _ on _\<close> 55)
+  | SporadicOnTvar     \<open>clock\<close> \<open>'\<tau> tag_expr\<close>  \<open>clock\<close>   (\<open>_ sporadic\<sharp> _ on _\<close> 55) 
+  | TagRelation        \<open>clock\<close> \<open>clock\<close> \<open>('\<tau> tag_const \<times> '\<tau> tag_const) \<Rightarrow> bool\<close> 
                                                       (\<open>time-relation \<lfloor>_, _\<rfloor> \<in> _\<close> 55)
-  | Implies          \<open>clock\<close> \<open>clock\<close>                  (infixr \<open>implies\<close> 55)
-  | ImpliesNot       \<open>clock\<close> \<open>clock\<close>                  (infixr \<open>implies not\<close> 55)
-  | TimeDelayedBy    \<open>clock\<close> \<open>'\<tau> tag_const\<close> \<open>clock\<close> \<open>clock\<close> (* Targets stutter-invariance *)
+  | Implies            \<open>clock\<close> \<open>clock\<close>                  (infixr \<open>implies\<close> 55)
+  | ImpliesNot         \<open>clock\<close> \<open>clock\<close>                  (infixr \<open>implies not\<close> 55)
+  | TimeDelayedBy      \<open>clock\<close> \<open>'\<tau> tag_const\<close> \<open>clock\<close> \<open>clock\<close> (* Targets stutter-invariance *)
                                                       (\<open>_ time-delayed by _ on _ implies _\<close> 55)
-  | TimeDelayedBy2   \<open>clock\<close> \<open>'\<tau> tag_const\<close> \<open>clock\<close> \<open>clock\<close> (* Targets operational semantics *)
-                                                      ("_ time-delayed2 by _ on _ implies _" 55)
+  | TimeDelayedByTvar   \<open>clock\<close> \<open>'\<tau> tag_const\<close> \<open>clock\<close> \<open>clock\<close> (* Targets operational semantics *)
+                                                      ("_ time-delayed\<sharp> by _ on _ implies _" 55)
                                                       
-  | WeaklyPrecedes   \<open>clock\<close> \<open>clock\<close>                  (infixr \<open>weakly precedes\<close> 55)
-  | StrictlyPrecedes \<open>clock\<close> \<open>clock\<close>                  (infixr \<open>strictly precedes\<close> 55)
-  | Kills            \<open>clock\<close> \<open>clock\<close>                  (infixr \<open>kills\<close> 55)
+  | WeaklyPrecedes     \<open>clock\<close> \<open>clock\<close>                  (infixr \<open>weakly precedes\<close> 55)
+  | StrictlyPrecedes   \<open>clock\<close> \<open>clock\<close>                  (infixr \<open>strictly precedes\<close> 55)
+  | Kills              \<open>clock\<close> \<open>clock\<close>                  (infixr \<open>kills\<close> 55)
 
 text\<open>
   A TESL formula is just a list of atomic constraints, with implicit conjunction
@@ -65,7 +63,7 @@ text\<open>
 \<close>
 fun positive_atom :: \<open>'\<tau> TESL_atomic \<Rightarrow> bool\<close> where
     \<open>positive_atom (_ sporadic _ on _) = True\<close>
-  | \<open>positive_atom (_ sporadic-add _ on _) = True\<close>
+  | \<open>positive_atom (_ sporadic\<sharp> _ on _) = True\<close>
   | \<open>positive_atom _                   = False\<close>
 
 text\<open>
@@ -245,5 +243,12 @@ begin
   qed
 
 end
+
+(* TODO: text *)
+fun suited_for_sttuter_inv_atom :: \<open>'\<tau> TESL_atomic \<Rightarrow> bool\<close> where
+    \<open>suited_for_sttuter_inv_atom (_ sporadic\<sharp> _ on _)                  = False\<close>
+  | \<open>suited_for_sttuter_inv_atom (_ time-delayed\<sharp> by _ on _ implies _) = False\<close>
+  | \<open>suited_for_sttuter_inv_atom _                                     = True\<close>
+
 
 end
