src/Denotational.thy
@@ -29,9 +29,9 @@ where
       instant where the time on @{term \<open>K\<^sub>2\<close>} is @{term \<open>\<tau>\<close>}.\<close>
     \<open>\<lbrakk> K\<^sub>1 sporadic \<tau> on K\<^sub>2 \<rbrakk>\<^sub>T\<^sub>E\<^sub>S\<^sub>L =
         {\<rho>. \<exists>n::nat. ticks ((Rep_run \<rho>) n K\<^sub>1) \<and> time ((Rep_run \<rho>) n K\<^sub>2) = \<tau>}\<close>
-  \<comment> \<open>@{term \<open>K\<^sub>1 sporadic-add \<lparr>\<tau>\<^sub>v\<^sub>a\<^sub>r(K\<^sub>p\<^sub>a\<^sub>s\<^sub>t, n\<^sub>p\<^sub>a\<^sub>s\<^sub>t) \<oplus> \<delta>\<tau>\<rparr> on K\<^sub>2\<close>} means that @{term \<open>K\<^sub>1\<close>} should tick at an 
+  \<comment> \<open>@{term \<open>K\<^sub>1 sporadic\<sharp> \<lparr>\<tau>\<^sub>v\<^sub>a\<^sub>r(K\<^sub>p\<^sub>a\<^sub>s\<^sub>t, n\<^sub>p\<^sub>a\<^sub>s\<^sub>t) \<oplus> \<delta>\<tau>\<rparr> on K\<^sub>2\<close>} means that @{term \<open>K\<^sub>1\<close>} should tick at an 
       instant where the time on @{term \<open>K\<^sub>2\<close>} is @{term \<open>\<lparr>\<tau>\<^sub>v\<^sub>a\<^sub>r(K\<^sub>p\<^sub>a\<^sub>s\<^sub>t, n\<^sub>p\<^sub>a\<^sub>s\<^sub>t) \<oplus> \<delta>\<tau>\<rparr>\<close>}.\<close>
-  | \<open>\<lbrakk> K\<^sub>1 sporadic-add \<lparr>\<tau>\<^sub>v\<^sub>a\<^sub>r(K\<^sub>p\<^sub>a\<^sub>s\<^sub>t, n\<^sub>p\<^sub>a\<^sub>s\<^sub>t) \<oplus> \<delta>\<tau>\<rparr> on K\<^sub>2 \<rbrakk>\<^sub>T\<^sub>E\<^sub>S\<^sub>L =
+  | \<open>\<lbrakk> K\<^sub>1 sporadic\<sharp> \<lparr>\<tau>\<^sub>v\<^sub>a\<^sub>r(K\<^sub>p\<^sub>a\<^sub>s\<^sub>t, n\<^sub>p\<^sub>a\<^sub>s\<^sub>t) \<oplus> \<delta>\<tau>\<rparr> on K\<^sub>2 \<rbrakk>\<^sub>T\<^sub>E\<^sub>S\<^sub>L =
         {\<rho>. \<exists>n::nat. ticks ((Rep_run \<rho>) n K\<^sub>1) \<and> time ((Rep_run \<rho>) n K\<^sub>2) = time ((Rep_run \<rho>) n\<^sub>p\<^sub>a\<^sub>s\<^sub>t K\<^sub>p\<^sub>a\<^sub>s\<^sub>t) + \<delta>\<tau> }\<close>
   \<comment> \<open>@{term \<open>time-relation \<lfloor>K\<^sub>1, K\<^sub>2\<rfloor> \<in> R\<close>} means that at each instant, the time 
       on @{term \<open>K\<^sub>1\<close>} and the time on @{term \<open>K\<^sub>2\<close>} are in relation~@{term \<open>R\<close>}.\<close>
@@ -61,10 +61,10 @@ where
                             \<longrightarrow> ticks ((Rep_run \<rho>) m slave)
                  )
         }\<close>
-  \<comment> \<open>@{term \<open>master time-delayed2 by \<delta>\<tau> on measuring implies slave\<close>} is similar
+  \<comment> \<open>@{term \<open>master time-delayed\<sharp> by \<delta>\<tau> on measuring implies slave\<close>} is similar
         but targets operational execution and allow time to stagnate before
         triggering slave  \<close>
-  | \<open>\<lbrakk> master time-delayed2 by \<delta>\<tau> on measuring implies slave \<rbrakk>\<^sub>T\<^sub>E\<^sub>S\<^sub>L =
+  | \<open>\<lbrakk> master time-delayed\<sharp> by \<delta>\<tau> on measuring implies slave \<rbrakk>\<^sub>T\<^sub>E\<^sub>S\<^sub>L =
     \<comment> \<open>
       When master ticks, let's call @{term \<open>t\<^sub>0\<close>} the current date on measuring. Then, 
       slave will be ticking whenever time @{term \<open>t\<^sub>0+\<delta>t\<close>} is measured on measuring.
