src/Hygge_Theory.thy
@@ -56,67 +56,67 @@ proof -
       fix  \<Gamma> n K\<^sub>1 \<tau> K\<^sub>2 \<Psi> \<Phi>
       assume \<open>(\<Gamma>\<^sub>1, n\<^sub>1 \<turnstile> \<Psi>\<^sub>1 \<triangleright> \<Phi>\<^sub>1) = (\<Gamma>, n \<turnstile> (K\<^sub>1 sporadic \<tau> on K\<^sub>2) # \<Psi> \<triangleright> \<Phi>)\<close>
       and \<open>(\<Gamma>\<^sub>2, n\<^sub>2 \<turnstile> \<Psi>\<^sub>2 \<triangleright> \<Phi>\<^sub>2) = (\<Gamma>, n \<turnstile> \<Psi> \<triangleright> ((K\<^sub>1 sporadic \<tau> on K\<^sub>2) # \<Phi>))\<close>
-      thus ?P using HeronConf_interp_stepwise_sporadicon_cases
-                    HeronConf_interpretation.simps by blast
+      thus ?P using configuration_interp_stepwise_sporadicon_cases
+                    configuration_interpretation.simps by blast
     next
       fix  \<Gamma> n K\<^sub>1 \<tau> K\<^sub>2 \<Psi> \<Phi>
       assume \<open>(\<Gamma>\<^sub>1, n\<^sub>1 \<turnstile> \<Psi>\<^sub>1 \<triangleright> \<Phi>\<^sub>1) = (\<Gamma>, n \<turnstile> (K\<^sub>1 sporadic \<tau> on K\<^sub>2) # \<Psi> \<triangleright> \<Phi>)\<close>
       and \<open>(\<Gamma>\<^sub>2, n\<^sub>2 \<turnstile> \<Psi>\<^sub>2 \<triangleright> \<Phi>\<^sub>2) = (((K\<^sub>1 \<Up> n) # (K\<^sub>2 \<Down> n @ \<tau>) # \<Gamma>), n \<turnstile> \<Psi> \<triangleright> \<Phi>)\<close>
-      thus ?P using HeronConf_interp_stepwise_sporadicon_cases
-                    HeronConf_interpretation.simps by blast
+      thus ?P using configuration_interp_stepwise_sporadicon_cases
+                    configuration_interpretation.simps by blast
     next
       fix \<Gamma> n K\<^sub>1 \<tau>\<^sub>e\<^sub>x\<^sub>p\<^sub>r K\<^sub>2 \<Psi> \<Phi>
-      assume \<open>\<Gamma>\<^sub>1, n\<^sub>1 \<turnstile> \<Psi>\<^sub>1 \<triangleright> \<Phi>\<^sub>1 = \<Gamma>, n \<turnstile> (K\<^sub>1 sporadic-add \<tau>\<^sub>e\<^sub>x\<^sub>p\<^sub>r on K\<^sub>2) # \<Psi> \<triangleright> \<Phi>\<close>
-      and \<open>\<Gamma>\<^sub>2, n\<^sub>2 \<turnstile> \<Psi>\<^sub>2 \<triangleright> \<Phi>\<^sub>2 = \<Gamma>, n \<turnstile> \<Psi> \<triangleright> (K\<^sub>1 sporadic-add \<tau>\<^sub>e\<^sub>x\<^sub>p\<^sub>r on K\<^sub>2) # \<Phi>\<close>
-      thus ?P using HeronConf_interp_stepwise_sporadicon_add_cases
-                    HeronConf_interpretation.simps by blast
+      assume \<open>\<Gamma>\<^sub>1, n\<^sub>1 \<turnstile> \<Psi>\<^sub>1 \<triangleright> \<Phi>\<^sub>1 = \<Gamma>, n \<turnstile> (K\<^sub>1 sporadic\<sharp> \<tau>\<^sub>e\<^sub>x\<^sub>p\<^sub>r on K\<^sub>2) # \<Psi> \<triangleright> \<Phi>\<close>
+      and \<open>\<Gamma>\<^sub>2, n\<^sub>2 \<turnstile> \<Psi>\<^sub>2 \<triangleright> \<Phi>\<^sub>2 = \<Gamma>, n \<turnstile> \<Psi> \<triangleright> (K\<^sub>1 sporadic\<sharp> \<tau>\<^sub>e\<^sub>x\<^sub>p\<^sub>r on K\<^sub>2) # \<Phi>\<close>
+      thus ?P using configuration_interp_stepwise_sporadicon_tvar_cases
+                    configuration_interpretation.simps by blast
     next
       fix \<Gamma> n K\<^sub>1 \<tau>\<^sub>e\<^sub>x\<^sub>p\<^sub>r K\<^sub>2 \<Psi> \<Phi>
-      assume \<open>\<Gamma>\<^sub>1, n\<^sub>1 \<turnstile> \<Psi>\<^sub>1 \<triangleright> \<Phi>\<^sub>1 = \<Gamma>, n \<turnstile> (K\<^sub>1 sporadic-add \<tau>\<^sub>e\<^sub>x\<^sub>p\<^sub>r on K\<^sub>2) # \<Psi> \<triangleright> \<Phi>\<close>
-      and \<open>\<Gamma>\<^sub>2, n\<^sub>2 \<turnstile> \<Psi>\<^sub>2 \<triangleright> \<Phi>\<^sub>2 = K\<^sub>1 \<Up> n # K\<^sub>2 \<Down> n @@ \<tau>\<^sub>e\<^sub>x\<^sub>p\<^sub>r # \<Gamma>, n \<turnstile> \<Psi> \<triangleright> \<Phi>\<close>
-      thus ?P using HeronConf_interp_stepwise_sporadicon_add_cases
-                    HeronConf_interpretation.simps by blast
+      assume \<open>\<Gamma>\<^sub>1, n\<^sub>1 \<turnstile> \<Psi>\<^sub>1 \<triangleright> \<Phi>\<^sub>1 = \<Gamma>, n \<turnstile> (K\<^sub>1 sporadic\<sharp> \<tau>\<^sub>e\<^sub>x\<^sub>p\<^sub>r on K\<^sub>2) # \<Psi> \<triangleright> \<Phi>\<close>
+      and \<open>\<Gamma>\<^sub>2, n\<^sub>2 \<turnstile> \<Psi>\<^sub>2 \<triangleright> \<Phi>\<^sub>2 = K\<^sub>1 \<Up> n # K\<^sub>2 \<Down> n @\<sharp> \<tau>\<^sub>e\<^sub>x\<^sub>p\<^sub>r # \<Gamma>, n \<turnstile> \<Psi> \<triangleright> \<Phi>\<close>
+      thus ?P using configuration_interp_stepwise_sporadicon_tvar_cases
+                    configuration_interpretation.simps by blast
     next
       fix \<Gamma> n K\<^sub>1 K\<^sub>2 R \<Psi> \<Phi>
       assume \<open>(\<Gamma>\<^sub>1, n\<^sub>1 \<turnstile> \<Psi>\<^sub>1 \<triangleright> \<Phi>\<^sub>1) = (\<Gamma>, n \<turnstile> (time-relation \<lfloor>K\<^sub>1, K\<^sub>2\<rfloor> \<in> R) # \<Psi> \<triangleright> \<Phi>)\<close>
       and \<open>(\<Gamma>\<^sub>2, n\<^sub>2 \<turnstile> \<Psi>\<^sub>2 \<triangleright> \<Phi>\<^sub>2) = (((\<lfloor>\<tau>\<^sub>v\<^sub>a\<^sub>r (K\<^sub>1, n), \<tau>\<^sub>v\<^sub>a\<^sub>r (K\<^sub>2, n)\<rfloor> \<in> R) # \<Gamma>), n
                                       \<turnstile> \<Psi> \<triangleright> ((time-relation \<lfloor>K\<^sub>1, K\<^sub>2\<rfloor> \<in> R) # \<Phi>))\<close>
-      thus ?P using HeronConf_interp_stepwise_tagrel_cases
-                    HeronConf_interpretation.simps by blast
+      thus ?P using configuration_interp_stepwise_tagrel_cases
+                    configuration_interpretation.simps by blast
     next
       fix \<Gamma> n K\<^sub>1 K\<^sub>2 \<Psi> \<Phi>
       assume \<open>(\<Gamma>\<^sub>1, n\<^sub>1 \<turnstile> \<Psi>\<^sub>1 \<triangleright> \<Phi>\<^sub>1) = (\<Gamma>, n \<turnstile> (K\<^sub>1 implies K\<^sub>2) # \<Psi> \<triangleright> \<Phi>)\<close>
       and \<open>(\<Gamma>\<^sub>2, n\<^sub>2 \<turnstile> \<Psi>\<^sub>2 \<triangleright> \<Phi>\<^sub>2) = (((K\<^sub>1 \<not>\<Up> n) # \<Gamma>), n \<turnstile> \<Psi> \<triangleright> ((K\<^sub>1 implies K\<^sub>2) # \<Phi>))\<close>
-      thus ?P using HeronConf_interp_stepwise_implies_cases
-                    HeronConf_interpretation.simps by blast
+      thus ?P using configuration_interp_stepwise_implies_cases
+                    configuration_interpretation.simps by blast
     next
       fix \<Gamma> n K\<^sub>1 K\<^sub>2 \<Psi> \<Phi>
       assume \<open>(\<Gamma>\<^sub>1, n\<^sub>1 \<turnstile> \<Psi>\<^sub>1 \<triangleright> \<Phi>\<^sub>1) = (\<Gamma>, n \<turnstile> ((K\<^sub>1 implies K\<^sub>2) # \<Psi>) \<triangleright> \<Phi>)\<close>
       and \<open>(\<Gamma>\<^sub>2, n\<^sub>2 \<turnstile> \<Psi>\<^sub>2 \<triangleright> \<Phi>\<^sub>2) = (((K\<^sub>1 \<Up> n) # (K\<^sub>2 \<Up> n) # \<Gamma>), n
                                    \<turnstile> \<Psi> \<triangleright> ((K\<^sub>1 implies K\<^sub>2) # \<Phi>))\<close>
-      thus ?P using HeronConf_interp_stepwise_implies_cases
-                    HeronConf_interpretation.simps by blast
+      thus ?P using configuration_interp_stepwise_implies_cases
+                    configuration_interpretation.simps by blast
     next
       fix \<Gamma> n K\<^sub>1 K\<^sub>2 \<Psi> \<Phi>
       assume \<open>(\<Gamma>\<^sub>1, n\<^sub>1 \<turnstile> \<Psi>\<^sub>1 \<triangleright> \<Phi>\<^sub>1) = (\<Gamma>, n \<turnstile> ((K\<^sub>1 implies not K\<^sub>2) # \<Psi>) \<triangleright> \<Phi>)\<close>
       and \<open>(\<Gamma>\<^sub>2, n\<^sub>2 \<turnstile> \<Psi>\<^sub>2 \<triangleright> \<Phi>\<^sub>2) = (((K\<^sub>1 \<not>\<Up> n) # \<Gamma>), n \<turnstile> \<Psi> \<triangleright> ((K\<^sub>1 implies not K\<^sub>2) # \<Phi>))\<close>
-      thus ?P using HeronConf_interp_stepwise_implies_not_cases
-                    HeronConf_interpretation.simps by blast
+      thus ?P using configuration_interp_stepwise_implies_not_cases
+                    configuration_interpretation.simps by blast
     next
       fix \<Gamma> n K\<^sub>1 K\<^sub>2 \<Psi> \<Phi>
       assume \<open>(\<Gamma>\<^sub>1, n\<^sub>1 \<turnstile> \<Psi>\<^sub>1 \<triangleright> \<Phi>\<^sub>1) = (\<Gamma>, n \<turnstile> ((K\<^sub>1 implies not K\<^sub>2) # \<Psi>) \<triangleright> \<Phi>)\<close>
       and \<open>(\<Gamma>\<^sub>2, n\<^sub>2 \<turnstile> \<Psi>\<^sub>2 \<triangleright> \<Phi>\<^sub>2) = (((K\<^sub>1 \<Up> n) # (K\<^sub>2 \<not>\<Up> n) # \<Gamma>), n
                                    \<turnstile> \<Psi> \<triangleright> ((K\<^sub>1 implies not K\<^sub>2) # \<Phi>))\<close>
-      thus ?P using HeronConf_interp_stepwise_implies_not_cases
-                    HeronConf_interpretation.simps by blast
+      thus ?P using configuration_interp_stepwise_implies_not_cases
+                    configuration_interpretation.simps by blast
     next
       fix \<Gamma> n K\<^sub>1 \<delta>\<tau> K\<^sub>2 K\<^sub>3 \<Psi> \<Phi>
       assume \<open>(\<Gamma>\<^sub>1, n\<^sub>1 \<turnstile> \<Psi>\<^sub>1 \<triangleright> \<Phi>\<^sub>1) =
                 (\<Gamma>, n \<turnstile> ((K\<^sub>1 time-delayed by \<delta>\<tau> on K\<^sub>2 implies K\<^sub>3) # \<Psi>) \<triangleright> \<Phi>)\<close>
       and \<open>(\<Gamma>\<^sub>2, n\<^sub>2 \<turnstile> \<Psi>\<^sub>2 \<triangleright> \<Phi>\<^sub>2) =
             (((K\<^sub>1 \<not>\<Up> n) # \<Gamma>), n \<turnstile> \<Psi> \<triangleright> ((K\<^sub>1 time-delayed by \<delta>\<tau> on K\<^sub>2 implies K\<^sub>3) # \<Phi>))\<close>
-      thus ?P using HeronConf_interp_stepwise_timedelayed_cases
-                    HeronConf_interpretation.simps by blast
+      thus ?P using configuration_interp_stepwise_timedelayed_cases
+                    configuration_interpretation.simps by blast
     next
       fix \<Gamma> n K\<^sub>1 \<delta>\<tau> K\<^sub>2 K\<^sub>3 \<Psi> \<Phi>
       assume \<open>(\<Gamma>\<^sub>1, n\<^sub>1 \<turnstile> \<Psi>\<^sub>1 \<triangleright> \<Phi>\<^sub>1) =
@@ -124,48 +124,48 @@ proof -
       and \<open>(\<Gamma>\<^sub>2, n\<^sub>2 \<turnstile> \<Psi>\<^sub>2 \<triangleright> \<Phi>\<^sub>2)
             = (((K\<^sub>1 \<Up> n) # (K\<^sub>2 @ n \<oplus> \<delta>\<tau> \<Rightarrow> K\<^sub>3) # \<Gamma>), n
                 \<turnstile> \<Psi> \<triangleright> ((K\<^sub>1 time-delayed by \<delta>\<tau> on K\<^sub>2 implies K\<^sub>3) # \<Phi>))\<close>
-      thus ?P using HeronConf_interp_stepwise_timedelayed_cases
-                    HeronConf_interpretation.simps by blast
+      thus ?P using configuration_interp_stepwise_timedelayed_cases
+                    configuration_interpretation.simps by blast
     next
       fix \<Gamma> n K\<^sub>1 \<delta>\<tau> K\<^sub>2 K\<^sub>3 \<Psi> \<Phi>
-      assume \<open>\<Gamma>\<^sub>1, n\<^sub>1 \<turnstile> \<Psi>\<^sub>1 \<triangleright> \<Phi>\<^sub>1 = \<Gamma>, n \<turnstile> (K\<^sub>1 time-delayed2 by \<delta>\<tau> on K\<^sub>2 implies K\<^sub>3) # \<Psi> \<triangleright> \<Phi>\<close>
-      and \<open>\<Gamma>\<^sub>2, n\<^sub>2 \<turnstile> \<Psi>\<^sub>2 \<triangleright> \<Phi>\<^sub>2 = K\<^sub>1 \<not>\<Up> n # \<Gamma>, n \<turnstile> \<Psi> \<triangleright> (K\<^sub>1 time-delayed2 by \<delta>\<tau> on K\<^sub>2 implies K\<^sub>3) # \<Phi>\<close>
-      thus ?P using HeronConf_interp_stepwise_timedelayed2_cases
-                    HeronConf_interpretation.simps by blast
+      assume \<open>\<Gamma>\<^sub>1, n\<^sub>1 \<turnstile> \<Psi>\<^sub>1 \<triangleright> \<Phi>\<^sub>1 = \<Gamma>, n \<turnstile> (K\<^sub>1 time-delayed\<sharp> by \<delta>\<tau> on K\<^sub>2 implies K\<^sub>3) # \<Psi> \<triangleright> \<Phi>\<close>
+      and \<open>\<Gamma>\<^sub>2, n\<^sub>2 \<turnstile> \<Psi>\<^sub>2 \<triangleright> \<Phi>\<^sub>2 = K\<^sub>1 \<not>\<Up> n # \<Gamma>, n \<turnstile> \<Psi> \<triangleright> (K\<^sub>1 time-delayed\<sharp> by \<delta>\<tau> on K\<^sub>2 implies K\<^sub>3) # \<Phi>\<close>
+      thus ?P using configuration_interp_stepwise_timedelayed_tvar_cases
+                    configuration_interpretation.simps by blast
     next
       fix \<Gamma> n K\<^sub>1 \<delta>\<tau> K\<^sub>2 K\<^sub>3 \<Psi> \<Phi>
-      assume \<open>\<Gamma>\<^sub>1, n\<^sub>1 \<turnstile> \<Psi>\<^sub>1 \<triangleright> \<Phi>\<^sub>1 = \<Gamma>, n \<turnstile> (K\<^sub>1 time-delayed2 by \<delta>\<tau> on K\<^sub>2 implies K\<^sub>3) # \<Psi> \<triangleright> \<Phi>\<close>
-      and \<open>\<Gamma>\<^sub>2, n\<^sub>2 \<turnstile> \<Psi>\<^sub>2 \<triangleright> \<Phi>\<^sub>2 = K\<^sub>1 \<Up> n # \<Gamma>, n \<turnstile> (K\<^sub>3 sporadic-add \<lparr> \<tau>\<^sub>v\<^sub>a\<^sub>r (K\<^sub>2, n) \<oplus> \<delta>\<tau> \<rparr> on K\<^sub>2) #
-               \<Psi> \<triangleright> (K\<^sub>1 time-delayed2 by \<delta>\<tau> on K\<^sub>2 implies K\<^sub>3) # \<Phi>\<close>
-      thus ?P using HeronConf_interp_stepwise_timedelayed2_cases
-                    HeronConf_interpretation.simps by blast
+      assume \<open>\<Gamma>\<^sub>1, n\<^sub>1 \<turnstile> \<Psi>\<^sub>1 \<triangleright> \<Phi>\<^sub>1 = \<Gamma>, n \<turnstile> (K\<^sub>1 time-delayed\<sharp> by \<delta>\<tau> on K\<^sub>2 implies K\<^sub>3) # \<Psi> \<triangleright> \<Phi>\<close>
+      and \<open>\<Gamma>\<^sub>2, n\<^sub>2 \<turnstile> \<Psi>\<^sub>2 \<triangleright> \<Phi>\<^sub>2 = K\<^sub>1 \<Up> n # \<Gamma>, n \<turnstile> (K\<^sub>3 sporadic\<sharp> \<lparr> \<tau>\<^sub>v\<^sub>a\<^sub>r (K\<^sub>2, n) \<oplus> \<delta>\<tau> \<rparr> on K\<^sub>2) #
+               \<Psi> \<triangleright> (K\<^sub>1 time-delayed\<sharp> by \<delta>\<tau> on K\<^sub>2 implies K\<^sub>3) # \<Phi>\<close>
+      thus ?P using configuration_interp_stepwise_timedelayed_tvar_cases
+                    configuration_interpretation.simps by blast
     next
       fix \<Gamma> n K\<^sub>1 K\<^sub>2 \<Psi> \<Phi>
       assume \<open>(\<Gamma>\<^sub>1, n\<^sub>1 \<turnstile> \<Psi>\<^sub>1 \<triangleright> \<Phi>\<^sub>1) = (\<Gamma>, n \<turnstile> ((K\<^sub>1 weakly precedes K\<^sub>2) # \<Psi>) \<triangleright> \<Phi>)\<close>
       and \<open>(\<Gamma>\<^sub>2, n\<^sub>2 \<turnstile> \<Psi>\<^sub>2 \<triangleright> \<Phi>\<^sub>2) = (((\<lceil>#\<^sup>\<le> K\<^sub>2 n, #\<^sup>\<le> K\<^sub>1 n\<rceil> \<in> (\<lambda>(x, y). x \<le> y)) # \<Gamma>), n
                                   \<turnstile> \<Psi> \<triangleright> ((K\<^sub>1 weakly precedes K\<^sub>2) # \<Phi>))\<close>
-      thus ?P using HeronConf_interp_stepwise_weakly_precedes_cases
-                    HeronConf_interpretation.simps by blast
+      thus ?P using configuration_interp_stepwise_weakly_precedes_cases
+                    configuration_interpretation.simps by blast
     next
       fix \<Gamma> n K\<^sub>1 K\<^sub>2 \<Psi> \<Phi>
       assume \<open>(\<Gamma>\<^sub>1, n\<^sub>1 \<turnstile> \<Psi>\<^sub>1 \<triangleright> \<Phi>\<^sub>1) = (\<Gamma>, n \<turnstile> ((K\<^sub>1 strictly precedes K\<^sub>2) # \<Psi>) \<triangleright> \<Phi>)\<close>
       and \<open>(\<Gamma>\<^sub>2, n\<^sub>2 \<turnstile> \<Psi>\<^sub>2 \<triangleright> \<Phi>\<^sub>2) = (((\<lceil>#\<^sup>\<le> K\<^sub>2 n, #\<^sup>< K\<^sub>1 n\<rceil> \<in> (\<lambda>(x, y). x \<le> y)) # \<Gamma>), n
                                   \<turnstile> \<Psi> \<triangleright> ((K\<^sub>1 strictly precedes K\<^sub>2) # \<Phi>))\<close>
-      thus ?P using HeronConf_interp_stepwise_strictly_precedes_cases
-                    HeronConf_interpretation.simps by blast
+      thus ?P using configuration_interp_stepwise_strictly_precedes_cases
+                    configuration_interpretation.simps by blast
     next
       fix \<Gamma> n K\<^sub>1 K\<^sub>2 \<Psi> \<Phi>
       assume \<open>(\<Gamma>\<^sub>1, n\<^sub>1 \<turnstile> \<Psi>\<^sub>1 \<triangleright> \<Phi>\<^sub>1) = (\<Gamma>, n \<turnstile> ((K\<^sub>1 kills K\<^sub>2) # \<Psi>) \<triangleright> \<Phi>)\<close>
       and \<open>(\<Gamma>\<^sub>2, n\<^sub>2 \<turnstile> \<Psi>\<^sub>2 \<triangleright> \<Phi>\<^sub>2) = (((K\<^sub>1 \<not>\<Up> n) # \<Gamma>), n \<turnstile> \<Psi> \<triangleright> ((K\<^sub>1 kills K\<^sub>2) # \<Phi>))\<close>
-      thus ?P using HeronConf_interp_stepwise_kills_cases
-                    HeronConf_interpretation.simps by blast
+      thus ?P using configuration_interp_stepwise_kills_cases
+                    configuration_interpretation.simps by blast
     next
       fix \<Gamma> n K\<^sub>1 K\<^sub>2 \<Psi> \<Phi>
       assume \<open>(\<Gamma>\<^sub>1, n\<^sub>1 \<turnstile> \<Psi>\<^sub>1 \<triangleright> \<Phi>\<^sub>1) = (\<Gamma>, n \<turnstile> ((K\<^sub>1 kills K\<^sub>2) # \<Psi>) \<triangleright> \<Phi>)\<close>
       and \<open>(\<Gamma>\<^sub>2, n\<^sub>2 \<turnstile> \<Psi>\<^sub>2 \<triangleright> \<Phi>\<^sub>2) =
             (((K\<^sub>1 \<Up> n) # (K\<^sub>2 \<not>\<Up> \<ge> n) # \<Gamma>), n \<turnstile> \<Psi> \<triangleright> ((K\<^sub>1 kills K\<^sub>2) # \<Phi>))\<close>
-      thus ?P using HeronConf_interp_stepwise_kills_cases
-                    HeronConf_interpretation.simps by blast
+      thus ?P using configuration_interp_stepwise_kills_cases
+                    configuration_interpretation.simps by blast
     qed
   qed
 qed
@@ -231,62 +231,62 @@ lemma complete_direct_successors:
   proof (induct \<Psi>)
     case Nil
     show ?case
-      using HeronConf_interp_stepwise_instant_cases operational_semantics_step.simps
+      using configuration_interp_stepwise_instant_cases operational_semantics_step.simps
             operational_semantics_intro.instant_i
       by fastforce
   next
     case (Cons \<psi> \<Psi>)  thus ?case
       proof (cases \<psi>)
         case (SporadicOn K1 \<tau> K2) thus ?thesis 
-          using HeronConf_interp_stepwise_sporadicon_cases
+          using configuration_interp_stepwise_sporadicon_cases
                                       [of \<open>\<Gamma>\<close> \<open>n\<close> \<open>K1\<close> \<open>\<tau>\<close> \<open>K2\<close> \<open>\<Psi>\<close> \<open>\<Phi>\<close>]
                 Cnext_solve_sporadicon[of \<open>\<Gamma>\<close> \<open>n\<close> \<open>\<Psi>\<close> \<open>K1\<close> \<open>\<tau>\<close> \<open>K2\<close> \<open>\<Phi>\<close>] by blast
       next
-        case (SporadicAdd X1 X2 X3) thus ?thesis
-          using HeronConf_interp_stepwise_sporadicon_add_cases
-                Cnext_solve_sporadicon_add
-          by (metis (mono_tags, lifting) SUP_upper Un_subset_iff elims_part mem_Collect_eq sporadic_add_e1 sporadic_add_e2)
+        case (SporadicOnTvar X1 X2 X3) thus ?thesis
+          using configuration_interp_stepwise_sporadicon_tvar_cases
+                Cnext_solve_sporadicon_tvar
+          by (metis (mono_tags, lifting) SUP_upper Un_subset_iff elims_part mem_Collect_eq sporadic_on_tvar_e1 sporadic_on_tvar_e2)
       next
         case (TagRelation K\<^sub>1 K\<^sub>2 R) thus ?thesis
-          using HeronConf_interp_stepwise_tagrel_cases
+          using configuration_interp_stepwise_tagrel_cases
                                   [of \<open>\<Gamma>\<close> \<open>n\<close> \<open>K\<^sub>1\<close> \<open>K\<^sub>2\<close> \<open>R\<close> \<open>\<Psi>\<close> \<open>\<Phi>\<close>]
                 Cnext_solve_tagrel[of \<open>K\<^sub>1\<close> \<open>n\<close> \<open>K\<^sub>2\<close> \<open>R\<close> \<open>\<Gamma>\<close> \<open>\<Psi>\<close> \<open>\<Phi>\<close>] by blast
       next
         case (Implies K1 K2) thus ?thesis
-          using HeronConf_interp_stepwise_implies_cases
+          using configuration_interp_stepwise_implies_cases
                                    [of \<open>\<Gamma>\<close> \<open>n\<close> \<open>K1\<close> \<open>K2\<close> \<open>\<Psi>\<close> \<open>\<Phi>\<close>]
                 Cnext_solve_implies[of \<open>K1\<close> \<open>n\<close> \<open>\<Gamma>\<close> \<open>\<Psi>\<close> \<open>K2\<close> \<open>\<Phi>\<close>] by blast
       next
         case (ImpliesNot K1 K2) thus ?thesis
-          using HeronConf_interp_stepwise_implies_not_cases
+          using configuration_interp_stepwise_implies_not_cases
                                        [of \<open>\<Gamma>\<close> \<open>n\<close> \<open>K1\<close> \<open>K2\<close> \<open>\<Psi>\<close> \<open>\<Phi>\<close>]
                 Cnext_solve_implies_not[of \<open>K1\<close> \<open>n\<close> \<open>\<Gamma>\<close> \<open>\<Psi>\<close> \<open>K2\<close> \<open>\<Phi>\<close>] by blast
       next
         case (TimeDelayedBy Kmast \<tau> Kmeas Kslave) thus ?thesis
-          using HeronConf_interp_stepwise_timedelayed_cases
+          using configuration_interp_stepwise_timedelayed_cases
                           [of \<open>\<Gamma>\<close> \<open>n\<close> \<open>Kmast\<close> \<open>\<tau>\<close> \<open>Kmeas\<close> \<open>Kslave\<close> \<open>\<Psi>\<close> \<open>\<Phi>\<close>]
                 Cnext_solve_timedelayed
                           [of \<open>Kmast\<close> \<open>n\<close> \<open>\<Gamma>\<close> \<open>\<Psi>\<close> \<open>\<tau>\<close> \<open>Kmeas\<close> \<open>Kslave\<close> \<open>\<Phi>\<close>] by blast
       next
-        case (TimeDelayedBy2 Kmast \<tau> Kmeas Kslave) thus ?thesis
-          using HeronConf_interp_stepwise_timedelayed2_cases
-                Cnext_solve_timedelayed2
-          by (metis (mono_tags, lifting) SUP_upper Un_subset_iff elims_part mem_Collect_eq timedelayed2_e1 timedelayed2_e2)
+        case (TimeDelayedByTvar Kmast \<tau> Kmeas Kslave) thus ?thesis
+          using configuration_interp_stepwise_timedelayed_tvar_cases
+                Cnext_solve_timedelayed_tvar
+          by (metis (mono_tags, lifting) SUP_upper Un_subset_iff elims_part mem_Collect_eq timedelayed_tvar_e1 timedelayed_tvar_e2)
       next
         case (WeaklyPrecedes K1 K2) thus ?thesis
-          using HeronConf_interp_stepwise_weakly_precedes_cases
+          using configuration_interp_stepwise_weakly_precedes_cases
                                            [of \<open>\<Gamma>\<close> \<open>n\<close> \<open>K1\<close> \<open>K2\<close> \<open>\<Psi>\<close> \<open>\<Phi>\<close>]
                 Cnext_solve_weakly_precedes[of \<open>K2\<close> \<open>n\<close> \<open>K1\<close> \<open>\<Gamma>\<close> \<open>\<Psi>\<close>  \<open>\<Phi>\<close>]
           by blast
       next
         case (StrictlyPrecedes K1 K2)  thus ?thesis
-          using HeronConf_interp_stepwise_strictly_precedes_cases
+          using configuration_interp_stepwise_strictly_precedes_cases
                                              [of \<open>\<Gamma>\<close> \<open>n\<close> \<open>K1\<close> \<open>K2\<close> \<open>\<Psi>\<close> \<open>\<Phi>\<close>]
                 Cnext_solve_strictly_precedes[of \<open>K2\<close> \<open>n\<close> \<open>K1\<close> \<open>\<Gamma>\<close> \<open>\<Psi>\<close>  \<open>\<Phi>\<close>]
           by blast
       next
         case (Kills K1 K2) thus ?thesis
-          using HeronConf_interp_stepwise_kills_cases[of \<open>\<Gamma>\<close> \<open>n\<close> \<open>K1\<close> \<open>K2\<close> \<open>\<Psi>\<close> \<open>\<Phi>\<close>]
+          using configuration_interp_stepwise_kills_cases[of \<open>\<Gamma>\<close> \<open>n\<close> \<open>K1\<close> \<open>K2\<close> \<open>\<Psi>\<close> \<open>\<Phi>\<close>]
                 Cnext_solve_kills[of \<open>K1\<close> \<open>n\<close> \<open>\<Gamma>\<close> \<open>\<Psi>\<close> \<open>K2\<close> \<open>\<Phi>\<close>] by blast
       qed
   qed
@@ -294,7 +294,7 @@ lemma complete_direct_successors:
 lemma complete_direct_successors':
   shows \<open>\<lbrakk> \<S> \<rbrakk>\<^sub>c\<^sub>o\<^sub>n\<^sub>f\<^sub>i\<^sub>g \<subseteq> (\<Union>X\<in>\<C>\<^sub>n\<^sub>e\<^sub>x\<^sub>t \<S>. \<lbrakk> X \<rbrakk>\<^sub>c\<^sub>o\<^sub>n\<^sub>f\<^sub>i\<^sub>g)\<close>
 proof -
-  from HeronConf_interpretation.cases obtain \<Gamma> n \<Psi> \<Phi>
+  from configuration_interpretation.cases obtain \<Gamma> n \<Psi> \<Phi>
     where \<open>\<S> = (\<Gamma>, n \<turnstile> \<Psi> \<triangleright> \<Phi>)\<close> by blast
   with complete_direct_successors[of \<open>\<Gamma>\<close> \<open>n\<close> \<open>\<Psi>\<close> \<open>\<Phi>\<close>] show ?thesis by simp
 qed
@@ -368,7 +368,7 @@ next
         have branches: \<open>\<lbrakk> \<Gamma>, n \<turnstile> ((K\<^sub>1 sporadic \<tau> on K\<^sub>2) # \<Psi>) \<triangleright> \<Phi> \<rbrakk>\<^sub>c\<^sub>o\<^sub>n\<^sub>f\<^sub>i\<^sub>g
                       = \<lbrakk> \<Gamma>, n \<turnstile> \<Psi> \<triangleright> ((K\<^sub>1 sporadic \<tau> on K\<^sub>2) # \<Phi>) \<rbrakk>\<^sub>c\<^sub>o\<^sub>n\<^sub>f\<^sub>i\<^sub>g
                       \<union> \<lbrakk> ((K\<^sub>1 \<Up> n) # (K\<^sub>2 \<Down> n @ \<tau>) # \<Gamma>), n \<turnstile> \<Psi> \<triangleright> \<Phi> \<rbrakk>\<^sub>c\<^sub>o\<^sub>n\<^sub>f\<^sub>i\<^sub>g\<close>
-          using HeronConf_interp_stepwise_sporadicon_cases by simp
+          using configuration_interp_stepwise_sporadicon_cases by simp
         have br1: \<open>\<rho> \<in> \<lbrakk> \<Gamma>, n \<turnstile> \<Psi> \<triangleright> ((K\<^sub>1 sporadic \<tau> on K\<^sub>2) # \<Phi>) \<rbrakk>\<^sub>c\<^sub>o\<^sub>n\<^sub>f\<^sub>i\<^sub>g
                     \<Longrightarrow> \<exists>\<Gamma>\<^sub>k \<Psi>\<^sub>k \<Phi>\<^sub>k k.
                       ((\<Gamma>, n \<turnstile> ((K\<^sub>1 sporadic \<tau> on K\<^sub>2) # \<Psi>) \<triangleright> \<Phi>)
@@ -422,29 +422,29 @@ next
           by simp
         with br1 br2 show ?case by blast
     next
-      case (SporadicAdd K\<^sub>1 \<tau>\<^sub>e\<^sub>x\<^sub>p\<^sub>r K\<^sub>2)
-        have branches: \<open>\<lbrakk> \<Gamma>, n \<turnstile> ((K\<^sub>1 sporadic-add \<tau>\<^sub>e\<^sub>x\<^sub>p\<^sub>r on K\<^sub>2) # \<Psi>) \<triangleright> \<Phi> \<rbrakk>\<^sub>c\<^sub>o\<^sub>n\<^sub>f\<^sub>i\<^sub>g
-                      = \<lbrakk> \<Gamma>, n \<turnstile> \<Psi> \<triangleright> ((K\<^sub>1 sporadic-add \<tau>\<^sub>e\<^sub>x\<^sub>p\<^sub>r on K\<^sub>2) # \<Phi>) \<rbrakk>\<^sub>c\<^sub>o\<^sub>n\<^sub>f\<^sub>i\<^sub>g
-                      \<union> \<lbrakk> ((K\<^sub>1 \<Up> n) # (K\<^sub>2 \<Down> n @@ \<tau>\<^sub>e\<^sub>x\<^sub>p\<^sub>r) # \<Gamma>), n \<turnstile> \<Psi> \<triangleright> \<Phi> \<rbrakk>\<^sub>c\<^sub>o\<^sub>n\<^sub>f\<^sub>i\<^sub>g\<close>
-          using HeronConf_interp_stepwise_sporadicon_add_cases by simp
-        have br1: \<open>\<rho> \<in> \<lbrakk> \<Gamma>, n \<turnstile> \<Psi> \<triangleright> ((K\<^sub>1 sporadic-add \<tau>\<^sub>e\<^sub>x\<^sub>p\<^sub>r on K\<^sub>2) # \<Phi>) \<rbrakk>\<^sub>c\<^sub>o\<^sub>n\<^sub>f\<^sub>i\<^sub>g
+      case (SporadicOnTvar K\<^sub>1 \<tau>\<^sub>e\<^sub>x\<^sub>p\<^sub>r K\<^sub>2)
+        have branches: \<open>\<lbrakk> \<Gamma>, n \<turnstile> ((K\<^sub>1 sporadic\<sharp> \<tau>\<^sub>e\<^sub>x\<^sub>p\<^sub>r on K\<^sub>2) # \<Psi>) \<triangleright> \<Phi> \<rbrakk>\<^sub>c\<^sub>o\<^sub>n\<^sub>f\<^sub>i\<^sub>g
+                      = \<lbrakk> \<Gamma>, n \<turnstile> \<Psi> \<triangleright> ((K\<^sub>1 sporadic\<sharp> \<tau>\<^sub>e\<^sub>x\<^sub>p\<^sub>r on K\<^sub>2) # \<Phi>) \<rbrakk>\<^sub>c\<^sub>o\<^sub>n\<^sub>f\<^sub>i\<^sub>g
+                      \<union> \<lbrakk> ((K\<^sub>1 \<Up> n) # (K\<^sub>2 \<Down> n @\<sharp> \<tau>\<^sub>e\<^sub>x\<^sub>p\<^sub>r) # \<Gamma>), n \<turnstile> \<Psi> \<triangleright> \<Phi> \<rbrakk>\<^sub>c\<^sub>o\<^sub>n\<^sub>f\<^sub>i\<^sub>g\<close>
+          using configuration_interp_stepwise_sporadicon_tvar_cases by simp
+        have br1: \<open>\<rho> \<in> \<lbrakk> \<Gamma>, n \<turnstile> \<Psi> \<triangleright> ((K\<^sub>1 sporadic\<sharp> \<tau>\<^sub>e\<^sub>x\<^sub>p\<^sub>r on K\<^sub>2) # \<Phi>) \<rbrakk>\<^sub>c\<^sub>o\<^sub>n\<^sub>f\<^sub>i\<^sub>g
                     \<Longrightarrow> \<exists>\<Gamma>\<^sub>k \<Psi>\<^sub>k \<Phi>\<^sub>k k.
-                      ((\<Gamma>, n \<turnstile> ((K\<^sub>1 sporadic-add \<tau>\<^sub>e\<^sub>x\<^sub>p\<^sub>r on K\<^sub>2) # \<Psi>) \<triangleright> \<Phi>)
+                      ((\<Gamma>, n \<turnstile> ((K\<^sub>1 sporadic\<sharp> \<tau>\<^sub>e\<^sub>x\<^sub>p\<^sub>r on K\<^sub>2) # \<Psi>) \<triangleright> \<Phi>)
                           \<hookrightarrow>\<^bsup>k\<^esup> (\<Gamma>\<^sub>k, Suc n \<turnstile> \<Psi>\<^sub>k \<triangleright> \<Phi>\<^sub>k))
                       \<and> \<rho> \<in> \<lbrakk> \<Gamma>\<^sub>k, Suc n \<turnstile> \<Psi>\<^sub>k \<triangleright> \<Phi>\<^sub>k \<rbrakk>\<^sub>c\<^sub>o\<^sub>n\<^sub>f\<^sub>i\<^sub>g\<close>
-          by (meson Cons.hyps elims_part relpowp_Suc_I2 sporadic_add_e1)
-      moreover have br2: "\<rho> \<in> \<lbrakk> ((K\<^sub>1 \<Up> n) # (K\<^sub>2 \<Down> n @@ \<tau>\<^sub>e\<^sub>x\<^sub>p\<^sub>r) # \<Gamma>), n \<turnstile> \<Psi> \<triangleright> \<Phi> \<rbrakk>\<^sub>c\<^sub>o\<^sub>n\<^sub>f\<^sub>i\<^sub>g \<Longrightarrow> \<exists>\<Gamma>\<^sub>k \<Psi>\<^sub>k \<Phi>\<^sub>k k.
-                       ((\<Gamma>, n \<turnstile> ((K\<^sub>1 sporadic-add \<tau>\<^sub>e\<^sub>x\<^sub>p\<^sub>r on K\<^sub>2) # \<Psi>) \<triangleright> \<Phi>) \<hookrightarrow>\<^bsup>k\<^esup> (\<Gamma>\<^sub>k, Suc n \<turnstile> \<Psi>\<^sub>k \<triangleright> \<Phi>\<^sub>k))
+          by (meson Cons.hyps elims_part relpowp_Suc_I2 sporadic_on_tvar_e1)
+      moreover have br2: "\<rho> \<in> \<lbrakk> ((K\<^sub>1 \<Up> n) # (K\<^sub>2 \<Down> n @\<sharp> \<tau>\<^sub>e\<^sub>x\<^sub>p\<^sub>r) # \<Gamma>), n \<turnstile> \<Psi> \<triangleright> \<Phi> \<rbrakk>\<^sub>c\<^sub>o\<^sub>n\<^sub>f\<^sub>i\<^sub>g \<Longrightarrow> \<exists>\<Gamma>\<^sub>k \<Psi>\<^sub>k \<Phi>\<^sub>k k.
+                       ((\<Gamma>, n \<turnstile> ((K\<^sub>1 sporadic\<sharp> \<tau>\<^sub>e\<^sub>x\<^sub>p\<^sub>r on K\<^sub>2) # \<Psi>) \<triangleright> \<Phi>) \<hookrightarrow>\<^bsup>k\<^esup> (\<Gamma>\<^sub>k, Suc n \<turnstile> \<Psi>\<^sub>k \<triangleright> \<Phi>\<^sub>k))
                       \<and> \<rho> \<in> \<lbrakk> \<Gamma>\<^sub>k, Suc n \<turnstile> \<Psi>\<^sub>k \<triangleright> \<Phi>\<^sub>k \<rbrakk>\<^sub>c\<^sub>o\<^sub>n\<^sub>f\<^sub>i\<^sub>g"
-          by (meson Cons.hyps elims_part relpowp_Suc_I2 sporadic_add_e2)
+          by (meson Cons.hyps elims_part relpowp_Suc_I2 sporadic_on_tvar_e2)
         ultimately show ?case
-          by (metis SporadicAdd.prems(2) UnE branches)
+          by (metis SporadicOnTvar.prems(2) UnE branches)
   next
     case (TagRelation K\<^sub>1 K\<^sub>2 R)
       have branches: \<open>\<lbrakk> \<Gamma>, n \<turnstile> ((time-relation \<lfloor>K\<^sub>1, K\<^sub>2\<rfloor> \<in> R) # \<Psi>) \<triangleright> \<Phi> \<rbrakk>\<^sub>c\<^sub>o\<^sub>n\<^sub>f\<^sub>i\<^sub>g
           = \<lbrakk> ((\<lfloor>\<tau>\<^sub>v\<^sub>a\<^sub>r(K\<^sub>1, n), \<tau>\<^sub>v\<^sub>a\<^sub>r(K\<^sub>2, n)\<rfloor> \<in> R) # \<Gamma>), n
               \<turnstile> \<Psi> \<triangleright> ((time-relation \<lfloor>K\<^sub>1, K\<^sub>2\<rfloor> \<in> R) # \<Phi>) \<rbrakk>\<^sub>c\<^sub>o\<^sub>n\<^sub>f\<^sub>i\<^sub>g\<close>
-        using HeronConf_interp_stepwise_tagrel_cases by simp
+        using configuration_interp_stepwise_tagrel_cases by simp
       thus ?case
       proof -
         have \<open>\<exists>\<Gamma>\<^sub>k \<Psi>\<^sub>k \<Phi>\<^sub>k k.
@@ -472,7 +472,7 @@ next
       have branches: \<open>\<lbrakk> \<Gamma>, n \<turnstile> ((K\<^sub>1 implies K\<^sub>2) # \<Psi>) \<triangleright> \<Phi> \<rbrakk>\<^sub>c\<^sub>o\<^sub>n\<^sub>f\<^sub>i\<^sub>g
           = \<lbrakk> ((K\<^sub>1 \<not>\<Up> n) # \<Gamma>), n \<turnstile> \<Psi> \<triangleright> ((K\<^sub>1 implies K\<^sub>2) # \<Phi>) \<rbrakk>\<^sub>c\<^sub>o\<^sub>n\<^sub>f\<^sub>i\<^sub>g
           \<union> \<lbrakk> ((K\<^sub>1 \<Up> n) # (K\<^sub>2 \<Up> n) # \<Gamma>), n \<turnstile> \<Psi> \<triangleright> ((K\<^sub>1 implies K\<^sub>2) # \<Phi>) \<rbrakk>\<^sub>c\<^sub>o\<^sub>n\<^sub>f\<^sub>i\<^sub>g\<close>
-        using HeronConf_interp_stepwise_implies_cases by simp
+        using configuration_interp_stepwise_implies_cases by simp
       moreover have br1: \<open>\<rho> \<in> \<lbrakk> ((K\<^sub>1 \<not>\<Up> n) # \<Gamma>), n \<turnstile> \<Psi> \<triangleright> ((K\<^sub>1 implies K\<^sub>2) # \<Phi>) \<rbrakk>\<^sub>c\<^sub>o\<^sub>n\<^sub>f\<^sub>i\<^sub>g
                 \<Longrightarrow> \<exists>\<Gamma>\<^sub>k \<Psi>\<^sub>k \<Phi>\<^sub>k k. ((\<Gamma>, n \<turnstile> ((K\<^sub>1 implies K\<^sub>2) # \<Psi>) \<triangleright> \<Phi>)
                                     \<hookrightarrow>\<^bsup>k\<^esup> (\<Gamma>\<^sub>k, Suc n \<turnstile> \<Psi>\<^sub>k \<triangleright> \<Phi>\<^sub>k))
@@ -525,7 +525,7 @@ next
       have branches: \<open>\<lbrakk> \<Gamma>, n \<turnstile> ((K\<^sub>1 implies not K\<^sub>2) # \<Psi>) \<triangleright> \<Phi> \<rbrakk>\<^sub>c\<^sub>o\<^sub>n\<^sub>f\<^sub>i\<^sub>g
           = \<lbrakk> ((K\<^sub>1 \<not>\<Up> n) # \<Gamma>), n \<turnstile> \<Psi> \<triangleright> ((K\<^sub>1 implies not K\<^sub>2) # \<Phi>) \<rbrakk>\<^sub>c\<^sub>o\<^sub>n\<^sub>f\<^sub>i\<^sub>g
           \<union> \<lbrakk> ((K\<^sub>1 \<Up> n) # (K\<^sub>2 \<not>\<Up> n) # \<Gamma>), n \<turnstile> \<Psi> \<triangleright> ((K\<^sub>1 implies not K\<^sub>2) # \<Phi>) \<rbrakk>\<^sub>c\<^sub>o\<^sub>n\<^sub>f\<^sub>i\<^sub>g\<close>
-        using HeronConf_interp_stepwise_implies_not_cases by simp
+        using configuration_interp_stepwise_implies_not_cases by simp
       moreover have br1: \<open>\<rho> \<in> \<lbrakk> ((K\<^sub>1 \<not>\<Up> n) # \<Gamma>), n
                             \<turnstile> \<Psi> \<triangleright> ((K\<^sub>1 implies not K\<^sub>2) # \<Phi>) \<rbrakk>\<^sub>c\<^sub>o\<^sub>n\<^sub>f\<^sub>i\<^sub>g
                 \<Longrightarrow> \<exists>\<Gamma>\<^sub>k \<Psi>\<^sub>k \<Phi>\<^sub>k k. ((\<Gamma>, n \<turnstile> ((K\<^sub>1 implies not K\<^sub>2) # \<Psi>) \<triangleright> \<Phi>)
@@ -583,7 +583,7 @@ next
               \<turnstile> \<Psi> \<triangleright> ((K\<^sub>1 time-delayed by \<delta>\<tau> on K\<^sub>2 implies K\<^sub>3) # \<Phi>) \<rbrakk>\<^sub>c\<^sub>o\<^sub>n\<^sub>f\<^sub>i\<^sub>g
           \<union> \<lbrakk> ((K\<^sub>1 \<Up> n) # (K\<^sub>2 @ n \<oplus> \<delta>\<tau> \<Rightarrow> K\<^sub>3) # \<Gamma>), n
               \<turnstile> \<Psi> \<triangleright> ((K\<^sub>1 time-delayed by \<delta>\<tau> on K\<^sub>2 implies K\<^sub>3) # \<Phi>) \<rbrakk>\<^sub>c\<^sub>o\<^sub>n\<^sub>f\<^sub>i\<^sub>g\<close>
-        using HeronConf_interp_stepwise_timedelayed_cases by simp
+        using configuration_interp_stepwise_timedelayed_cases by simp
       moreover have br1:
         \<open>\<rho> \<in> \<lbrakk> ((K\<^sub>1 \<not>\<Up> n) # \<Gamma>), n
               \<turnstile> \<Psi> \<triangleright> ((K\<^sub>1 time-delayed by \<delta>\<tau> on K\<^sub>2 implies K\<^sub>3) # \<Phi>) \<rbrakk>\<^sub>c\<^sub>o\<^sub>n\<^sub>f\<^sub>i\<^sub>g
@@ -645,81 +645,81 @@ next
       qed
       ultimately show ?case using TimeDelayedBy.prems(2) by blast
   next
-    case (TimeDelayedBy2 K\<^sub>1 \<delta>\<tau> K\<^sub>2 K\<^sub>3)
+    case (TimeDelayedByTvar K\<^sub>1 \<delta>\<tau> K\<^sub>2 K\<^sub>3)
       have branches:
-        \<open>\<lbrakk> \<Gamma>, n \<turnstile> ((K\<^sub>1 time-delayed2 by \<delta>\<tau> on K\<^sub>2 implies K\<^sub>3) # \<Psi>) \<triangleright> \<Phi> \<rbrakk>\<^sub>c\<^sub>o\<^sub>n\<^sub>f\<^sub>i\<^sub>g
+        \<open>\<lbrakk> \<Gamma>, n \<turnstile> ((K\<^sub>1 time-delayed\<sharp> by \<delta>\<tau> on K\<^sub>2 implies K\<^sub>3) # \<Psi>) \<triangleright> \<Phi> \<rbrakk>\<^sub>c\<^sub>o\<^sub>n\<^sub>f\<^sub>i\<^sub>g
           = \<lbrakk> ((K\<^sub>1 \<not>\<Up> n) # \<Gamma>), n
-              \<turnstile> \<Psi> \<triangleright> ((K\<^sub>1 time-delayed2 by \<delta>\<tau> on K\<^sub>2 implies K\<^sub>3) # \<Phi>) \<rbrakk>\<^sub>c\<^sub>o\<^sub>n\<^sub>f\<^sub>i\<^sub>g
+              \<turnstile> \<Psi> \<triangleright> ((K\<^sub>1 time-delayed\<sharp> by \<delta>\<tau> on K\<^sub>2 implies K\<^sub>3) # \<Phi>) \<rbrakk>\<^sub>c\<^sub>o\<^sub>n\<^sub>f\<^sub>i\<^sub>g
           \<union> \<lbrakk> ((K\<^sub>1 \<Up> n) # \<Gamma>), n
-              \<turnstile> (K\<^sub>3 sporadic-add \<lparr>\<tau>\<^sub>v\<^sub>a\<^sub>r(K\<^sub>2, n) \<oplus> \<delta>\<tau>\<rparr> on K\<^sub>2) # \<Psi> \<triangleright> ((K\<^sub>1 time-delayed2 by \<delta>\<tau> on K\<^sub>2 implies K\<^sub>3) # \<Phi>) \<rbrakk>\<^sub>c\<^sub>o\<^sub>n\<^sub>f\<^sub>i\<^sub>g\<close>
-        using HeronConf_interp_stepwise_timedelayed2_cases by simp
+              \<turnstile> (K\<^sub>3 sporadic\<sharp> \<lparr>\<tau>\<^sub>v\<^sub>a\<^sub>r(K\<^sub>2, n) \<oplus> \<delta>\<tau>\<rparr> on K\<^sub>2) # \<Psi> \<triangleright> ((K\<^sub>1 time-delayed\<sharp> by \<delta>\<tau> on K\<^sub>2 implies K\<^sub>3) # \<Phi>) \<rbrakk>\<^sub>c\<^sub>o\<^sub>n\<^sub>f\<^sub>i\<^sub>g\<close>
+        using configuration_interp_stepwise_timedelayed_tvar_cases by simp
       have more_branches:
-                "\<lbrakk> ((K\<^sub>1 \<Up> n) # \<Gamma>), n \<turnstile> ((K\<^sub>3 sporadic-add \<lparr>\<tau>\<^sub>v\<^sub>a\<^sub>r(K\<^sub>2, n) \<oplus> \<delta>\<tau>\<rparr> on K\<^sub>2) # \<Psi>) \<triangleright> ((K\<^sub>1 time-delayed2 by \<delta>\<tau> on K\<^sub>2 implies K\<^sub>3) # \<Phi>) \<rbrakk>\<^sub>c\<^sub>o\<^sub>n\<^sub>f\<^sub>i\<^sub>g
-                  = \<lbrakk> ((K\<^sub>1 \<Up> n) # \<Gamma>), n \<turnstile> \<Psi> \<triangleright> ((K\<^sub>3 sporadic-add \<lparr>\<tau>\<^sub>v\<^sub>a\<^sub>r(K\<^sub>2, n) \<oplus> \<delta>\<tau>\<rparr> on K\<^sub>2) # (K\<^sub>1 time-delayed2 by \<delta>\<tau> on K\<^sub>2 implies K\<^sub>3) # \<Phi>) \<rbrakk>\<^sub>c\<^sub>o\<^sub>n\<^sub>f\<^sub>i\<^sub>g
-                  \<union> \<lbrakk> ((K\<^sub>3 \<Up> n) # (K\<^sub>2 \<Down> n @@ \<lparr>\<tau>\<^sub>v\<^sub>a\<^sub>r(K\<^sub>2, n) \<oplus> \<delta>\<tau>\<rparr>) # (K\<^sub>1 \<Up> n) # \<Gamma>), n \<turnstile> \<Psi> \<triangleright> ((K\<^sub>1 time-delayed2 by \<delta>\<tau> on K\<^sub>2 implies K\<^sub>3) # \<Phi>) \<rbrakk>\<^sub>c\<^sub>o\<^sub>n\<^sub>f\<^sub>i\<^sub>g"
-            using HeronConf_interp_stepwise_sporadicon_add_cases by blast
+                "\<lbrakk> ((K\<^sub>1 \<Up> n) # \<Gamma>), n \<turnstile> ((K\<^sub>3 sporadic\<sharp> \<lparr>\<tau>\<^sub>v\<^sub>a\<^sub>r(K\<^sub>2, n) \<oplus> \<delta>\<tau>\<rparr> on K\<^sub>2) # \<Psi>) \<triangleright> ((K\<^sub>1 time-delayed\<sharp> by \<delta>\<tau> on K\<^sub>2 implies K\<^sub>3) # \<Phi>) \<rbrakk>\<^sub>c\<^sub>o\<^sub>n\<^sub>f\<^sub>i\<^sub>g
+                  = \<lbrakk> ((K\<^sub>1 \<Up> n) # \<Gamma>), n \<turnstile> \<Psi> \<triangleright> ((K\<^sub>3 sporadic\<sharp> \<lparr>\<tau>\<^sub>v\<^sub>a\<^sub>r(K\<^sub>2, n) \<oplus> \<delta>\<tau>\<rparr> on K\<^sub>2) # (K\<^sub>1 time-delayed\<sharp> by \<delta>\<tau> on K\<^sub>2 implies K\<^sub>3) # \<Phi>) \<rbrakk>\<^sub>c\<^sub>o\<^sub>n\<^sub>f\<^sub>i\<^sub>g
+                  \<union> \<lbrakk> ((K\<^sub>3 \<Up> n) # (K\<^sub>2 \<Down> n @\<sharp> \<lparr>\<tau>\<^sub>v\<^sub>a\<^sub>r(K\<^sub>2, n) \<oplus> \<delta>\<tau>\<rparr>) # (K\<^sub>1 \<Up> n) # \<Gamma>), n \<turnstile> \<Psi> \<triangleright> ((K\<^sub>1 time-delayed\<sharp> by \<delta>\<tau> on K\<^sub>2 implies K\<^sub>3) # \<Phi>) \<rbrakk>\<^sub>c\<^sub>o\<^sub>n\<^sub>f\<^sub>i\<^sub>g"
+            using configuration_interp_stepwise_sporadicon_tvar_cases by blast
       moreover have br1:
         \<open>\<rho> \<in> \<lbrakk> ((K\<^sub>1 \<not>\<Up> n) # \<Gamma>), n
-              \<turnstile> \<Psi> \<triangleright> ((K\<^sub>1 time-delayed2 by \<delta>\<tau> on K\<^sub>2 implies K\<^sub>3) # \<Phi>) \<rbrakk>\<^sub>c\<^sub>o\<^sub>n\<^sub>f\<^sub>i\<^sub>g
+              \<turnstile> \<Psi> \<triangleright> ((K\<^sub>1 time-delayed\<sharp> by \<delta>\<tau> on K\<^sub>2 implies K\<^sub>3) # \<Phi>) \<rbrakk>\<^sub>c\<^sub>o\<^sub>n\<^sub>f\<^sub>i\<^sub>g
           \<Longrightarrow> \<exists>\<Gamma>\<^sub>k \<Psi>\<^sub>k \<Phi>\<^sub>k k.
-            ((\<Gamma>, n \<turnstile> ((K\<^sub>1 time-delayed2 by \<delta>\<tau> on K\<^sub>2 implies K\<^sub>3) # \<Psi>) \<triangleright> \<Phi>)
+            ((\<Gamma>, n \<turnstile> ((K\<^sub>1 time-delayed\<sharp> by \<delta>\<tau> on K\<^sub>2 implies K\<^sub>3) # \<Psi>) \<triangleright> \<Phi>)
                 \<hookrightarrow>\<^bsup>k\<^esup> (\<Gamma>\<^sub>k, Suc n \<turnstile> \<Psi>\<^sub>k \<triangleright> \<Phi>\<^sub>k))
             \<and> \<rho> \<in> \<lbrakk> \<Gamma>\<^sub>k, Suc n \<turnstile> \<Psi>\<^sub>k \<triangleright> \<Phi>\<^sub>k \<rbrakk>\<^sub>c\<^sub>o\<^sub>n\<^sub>f\<^sub>i\<^sub>g\<close>
       proof -
         assume h1: \<open>\<rho> \<in> \<lbrakk> ((K\<^sub>1 \<not>\<Up> n) # \<Gamma>), n
-                         \<turnstile> \<Psi> \<triangleright> ((K\<^sub>1 time-delayed2 by \<delta>\<tau> on K\<^sub>2 implies K\<^sub>3) # \<Phi>) \<rbrakk>\<^sub>c\<^sub>o\<^sub>n\<^sub>f\<^sub>i\<^sub>g\<close>
+                         \<turnstile> \<Psi> \<triangleright> ((K\<^sub>1 time-delayed\<sharp> by \<delta>\<tau> on K\<^sub>2 implies K\<^sub>3) # \<Phi>) \<rbrakk>\<^sub>c\<^sub>o\<^sub>n\<^sub>f\<^sub>i\<^sub>g\<close>
         then have \<open>\<exists>\<Gamma>\<^sub>k \<Psi>\<^sub>k \<Phi>\<^sub>k k.
-          ((((K\<^sub>1 \<not>\<Up> n) # \<Gamma>), n \<turnstile> \<Psi> \<triangleright> ((K\<^sub>1 time-delayed2 by \<delta>\<tau> on K\<^sub>2 implies K\<^sub>3) # \<Phi>))
+          ((((K\<^sub>1 \<not>\<Up> n) # \<Gamma>), n \<turnstile> \<Psi> \<triangleright> ((K\<^sub>1 time-delayed\<sharp> by \<delta>\<tau> on K\<^sub>2 implies K\<^sub>3) # \<Phi>))
             \<hookrightarrow>\<^bsup>k\<^esup> (\<Gamma>\<^sub>k, Suc n \<turnstile> \<Psi>\<^sub>k \<triangleright> \<Phi>\<^sub>k))
           \<and> \<rho> \<in> \<lbrakk> \<Gamma>\<^sub>k, Suc n \<turnstile> \<Psi>\<^sub>k \<triangleright> \<Phi>\<^sub>k \<rbrakk>\<^sub>c\<^sub>o\<^sub>n\<^sub>f\<^sub>i\<^sub>g\<close>
-          using h1 TimeDelayedBy2.prems by simp
+          using h1 TimeDelayedByTvar.prems by simp
         from this obtain \<Gamma>\<^sub>k \<Psi>\<^sub>k \<Phi>\<^sub>k k
           where fp:\<open>(((K\<^sub>1 \<not>\<Up> n) # \<Gamma>), n
-                      \<turnstile> \<Psi> \<triangleright> ((K\<^sub>1 time-delayed2 by \<delta>\<tau> on K\<^sub>2 implies K\<^sub>3) # \<Phi>))
+                      \<turnstile> \<Psi> \<triangleright> ((K\<^sub>1 time-delayed\<sharp> by \<delta>\<tau> on K\<^sub>2 implies K\<^sub>3) # \<Phi>))
                     \<hookrightarrow>\<^bsup>k\<^esup> (\<Gamma>\<^sub>k, Suc n \<turnstile> \<Psi>\<^sub>k \<triangleright> \<Phi>\<^sub>k)\<close>
             and rc:\<open>\<rho> \<in> \<lbrakk> \<Gamma>\<^sub>k, Suc n \<turnstile> \<Psi>\<^sub>k \<triangleright> \<Phi>\<^sub>k \<rbrakk>\<^sub>c\<^sub>o\<^sub>n\<^sub>f\<^sub>i\<^sub>g\<close> by blast
-        have \<open>(\<Gamma>, n \<turnstile> ((K\<^sub>1 time-delayed2 by \<delta>\<tau> on K\<^sub>2 implies K\<^sub>3) # \<Psi>) \<triangleright> \<Phi>)
+        have \<open>(\<Gamma>, n \<turnstile> ((K\<^sub>1 time-delayed\<sharp> by \<delta>\<tau> on K\<^sub>2 implies K\<^sub>3) # \<Psi>) \<triangleright> \<Phi>)
               \<hookrightarrow> (((K\<^sub>1 \<not>\<Up> n) # \<Gamma>), n
-                    \<turnstile> \<Psi> \<triangleright> ((K\<^sub>1 time-delayed2 by \<delta>\<tau> on K\<^sub>2 implies K\<^sub>3) # \<Phi>))\<close>
-          by (simp add: elims_part timedelayed2_e1)
-        hence \<open>(\<Gamma>, n \<turnstile> ((K\<^sub>1 time-delayed2 by \<delta>\<tau> on K\<^sub>2 implies K\<^sub>3) # \<Psi>) \<triangleright> \<Phi>)
+                    \<turnstile> \<Psi> \<triangleright> ((K\<^sub>1 time-delayed\<sharp> by \<delta>\<tau> on K\<^sub>2 implies K\<^sub>3) # \<Phi>))\<close>
+          by (simp add: elims_part timedelayed_tvar_e1)
+        hence \<open>(\<Gamma>, n \<turnstile> ((K\<^sub>1 time-delayed\<sharp> by \<delta>\<tau> on K\<^sub>2 implies K\<^sub>3) # \<Psi>) \<triangleright> \<Phi>)
                 \<hookrightarrow>\<^bsup>Suc k\<^esup> (\<Gamma>\<^sub>k, Suc n \<turnstile> \<Psi>\<^sub>k \<triangleright> \<Phi>\<^sub>k)\<close>
           using fp relpowp_Suc_I2 by auto
         with rc show ?thesis by blast
       qed
       moreover have br2:
-        \<open>\<rho> \<in> \<lbrakk> ((K\<^sub>1 \<Up> n) # \<Gamma>), n \<turnstile> \<Psi> \<triangleright> (K\<^sub>3 sporadic-add \<lparr>\<tau>\<^sub>v\<^sub>a\<^sub>r(K\<^sub>2, n) \<oplus> \<delta>\<tau>\<rparr> on K\<^sub>2) # ((K\<^sub>1 time-delayed2 by \<delta>\<tau> on K\<^sub>2 implies K\<^sub>3) # \<Phi>) \<rbrakk>\<^sub>c\<^sub>o\<^sub>n\<^sub>f\<^sub>i\<^sub>g
+        \<open>\<rho> \<in> \<lbrakk> ((K\<^sub>1 \<Up> n) # \<Gamma>), n \<turnstile> \<Psi> \<triangleright> (K\<^sub>3 sporadic\<sharp> \<lparr>\<tau>\<^sub>v\<^sub>a\<^sub>r(K\<^sub>2, n) \<oplus> \<delta>\<tau>\<rparr> on K\<^sub>2) # ((K\<^sub>1 time-delayed\<sharp> by \<delta>\<tau> on K\<^sub>2 implies K\<^sub>3) # \<Phi>) \<rbrakk>\<^sub>c\<^sub>o\<^sub>n\<^sub>f\<^sub>i\<^sub>g
           \<Longrightarrow> \<exists>\<Gamma>\<^sub>k \<Psi>\<^sub>k \<Phi>\<^sub>k k.
-              ((\<Gamma>, n \<turnstile> ((K\<^sub>1 time-delayed2 by \<delta>\<tau> on K\<^sub>2 implies K\<^sub>3) # \<Psi>) \<triangleright> \<Phi>) \<hookrightarrow>\<^bsup>k\<^esup> (\<Gamma>\<^sub>k, Suc n \<turnstile> \<Psi>\<^sub>k \<triangleright> \<Phi>\<^sub>k))
+              ((\<Gamma>, n \<turnstile> ((K\<^sub>1 time-delayed\<sharp> by \<delta>\<tau> on K\<^sub>2 implies K\<^sub>3) # \<Psi>) \<triangleright> \<Phi>) \<hookrightarrow>\<^bsup>k\<^esup> (\<Gamma>\<^sub>k, Suc n \<turnstile> \<Psi>\<^sub>k \<triangleright> \<Phi>\<^sub>k))
               \<and> \<rho> \<in> \<lbrakk> \<Gamma>\<^sub>k, Suc n \<turnstile> \<Psi>\<^sub>k \<triangleright> \<Phi>\<^sub>k \<rbrakk>\<^sub>c\<^sub>o\<^sub>n\<^sub>f\<^sub>i\<^sub>g\<close>
         proof -
-          assume h2: "\<rho> \<in> \<lbrakk> ((K\<^sub>1 \<Up> n) # \<Gamma>), n \<turnstile> \<Psi> \<triangleright> ((K\<^sub>3 sporadic-add \<lparr>\<tau>\<^sub>v\<^sub>a\<^sub>r(K\<^sub>2, n) \<oplus> \<delta>\<tau>\<rparr> on K\<^sub>2) # (K\<^sub>1 time-delayed2 by \<delta>\<tau> on K\<^sub>2 implies K\<^sub>3) # \<Phi>) \<rbrakk>\<^sub>c\<^sub>o\<^sub>n\<^sub>f\<^sub>i\<^sub>g"
-          then have "\<exists>\<Gamma>\<^sub>k \<Psi>\<^sub>k \<Phi>\<^sub>k k. ((((K\<^sub>1 \<Up> n) # \<Gamma>), n \<turnstile> \<Psi> \<triangleright> ((K\<^sub>3 sporadic-add \<lparr>\<tau>\<^sub>v\<^sub>a\<^sub>r(K\<^sub>2, n) \<oplus> \<delta>\<tau>\<rparr> on K\<^sub>2) # (K\<^sub>1 time-delayed2 by \<delta>\<tau> on K\<^sub>2 implies K\<^sub>3) # \<Phi>)) \<hookrightarrow>\<^bsup>k\<^esup> (\<Gamma>\<^sub>k, Suc n \<turnstile> \<Psi>\<^sub>k \<triangleright> \<Phi>\<^sub>k)) \<and> \<rho> \<in> \<lbrakk> \<Gamma>\<^sub>k, Suc n \<turnstile> \<Psi>\<^sub>k \<triangleright> \<Phi>\<^sub>k \<rbrakk>\<^sub>c\<^sub>o\<^sub>n\<^sub>f\<^sub>i\<^sub>g"
-            using h2 TimeDelayedBy2.prems by simp
+          assume h2: "\<rho> \<in> \<lbrakk> ((K\<^sub>1 \<Up> n) # \<Gamma>), n \<turnstile> \<Psi> \<triangleright> ((K\<^sub>3 sporadic\<sharp> \<lparr>\<tau>\<^sub>v\<^sub>a\<^sub>r(K\<^sub>2, n) \<oplus> \<delta>\<tau>\<rparr> on K\<^sub>2) # (K\<^sub>1 time-delayed\<sharp> by \<delta>\<tau> on K\<^sub>2 implies K\<^sub>3) # \<Phi>) \<rbrakk>\<^sub>c\<^sub>o\<^sub>n\<^sub>f\<^sub>i\<^sub>g"
+          then have "\<exists>\<Gamma>\<^sub>k \<Psi>\<^sub>k \<Phi>\<^sub>k k. ((((K\<^sub>1 \<Up> n) # \<Gamma>), n \<turnstile> \<Psi> \<triangleright> ((K\<^sub>3 sporadic\<sharp> \<lparr>\<tau>\<^sub>v\<^sub>a\<^sub>r(K\<^sub>2, n) \<oplus> \<delta>\<tau>\<rparr> on K\<^sub>2) # (K\<^sub>1 time-delayed\<sharp> by \<delta>\<tau> on K\<^sub>2 implies K\<^sub>3) # \<Phi>)) \<hookrightarrow>\<^bsup>k\<^esup> (\<Gamma>\<^sub>k, Suc n \<turnstile> \<Psi>\<^sub>k \<triangleright> \<Phi>\<^sub>k)) \<and> \<rho> \<in> \<lbrakk> \<Gamma>\<^sub>k, Suc n \<turnstile> \<Psi>\<^sub>k \<triangleright> \<Phi>\<^sub>k \<rbrakk>\<^sub>c\<^sub>o\<^sub>n\<^sub>f\<^sub>i\<^sub>g"
+            using h2 TimeDelayedByTvar.prems by simp
           then show ?thesis
-            by (meson elims_part relpowp_Suc_I2 timedelayed2_e2 sporadic_add_e1)
+            by (meson elims_part relpowp_Suc_I2 timedelayed_tvar_e2 sporadic_on_tvar_e1)
         qed
       moreover have br2':
-        "\<rho> \<in> \<lbrakk> ((K\<^sub>3 \<Up> n) # (K\<^sub>2 \<Down> n @@ \<lparr>\<tau>\<^sub>v\<^sub>a\<^sub>r(K\<^sub>2, n) \<oplus> \<delta>\<tau>\<rparr>) # (K\<^sub>1 \<Up> n) # \<Gamma>), n \<turnstile> \<Psi> \<triangleright> ((K\<^sub>1 time-delayed2 by \<delta>\<tau> on K\<^sub>2 implies K\<^sub>3) # \<Phi>) \<rbrakk>\<^sub>c\<^sub>o\<^sub>n\<^sub>f\<^sub>i\<^sub>g
+        "\<rho> \<in> \<lbrakk> ((K\<^sub>3 \<Up> n) # (K\<^sub>2 \<Down> n @\<sharp> \<lparr>\<tau>\<^sub>v\<^sub>a\<^sub>r(K\<^sub>2, n) \<oplus> \<delta>\<tau>\<rparr>) # (K\<^sub>1 \<Up> n) # \<Gamma>), n \<turnstile> \<Psi> \<triangleright> ((K\<^sub>1 time-delayed\<sharp> by \<delta>\<tau> on K\<^sub>2 implies K\<^sub>3) # \<Phi>) \<rbrakk>\<^sub>c\<^sub>o\<^sub>n\<^sub>f\<^sub>i\<^sub>g
           \<Longrightarrow> \<exists>\<Gamma>\<^sub>k \<Psi>\<^sub>k \<Phi>\<^sub>k k.
-           ((\<Gamma>, n \<turnstile> ((K\<^sub>1 time-delayed2 by \<delta>\<tau> on K\<^sub>2 implies K\<^sub>3) # \<Psi>) \<triangleright> \<Phi>) \<hookrightarrow>\<^bsup>k\<^esup> (\<Gamma>\<^sub>k, Suc n \<turnstile> \<Psi>\<^sub>k \<triangleright> \<Phi>\<^sub>k))
+           ((\<Gamma>, n \<turnstile> ((K\<^sub>1 time-delayed\<sharp> by \<delta>\<tau> on K\<^sub>2 implies K\<^sub>3) # \<Psi>) \<triangleright> \<Phi>) \<hookrightarrow>\<^bsup>k\<^esup> (\<Gamma>\<^sub>k, Suc n \<turnstile> \<Psi>\<^sub>k \<triangleright> \<Phi>\<^sub>k))
           \<and> \<rho> \<in> \<lbrakk> \<Gamma>\<^sub>k, Suc n \<turnstile> \<Psi>\<^sub>k \<triangleright> \<Phi>\<^sub>k \<rbrakk>\<^sub>c\<^sub>o\<^sub>n\<^sub>f\<^sub>i\<^sub>g"
         proof -
-          assume h2: "\<rho> \<in> \<lbrakk> ((K\<^sub>3 \<Up> n) # (K\<^sub>2 \<Down> n @@ \<lparr>\<tau>\<^sub>v\<^sub>a\<^sub>r(K\<^sub>2, n) \<oplus> \<delta>\<tau>\<rparr>) # (K\<^sub>1 \<Up> n) # \<Gamma>), n \<turnstile> \<Psi> \<triangleright> ((K\<^sub>1 time-delayed2 by \<delta>\<tau> on K\<^sub>2 implies K\<^sub>3) # \<Phi>) \<rbrakk>\<^sub>c\<^sub>o\<^sub>n\<^sub>f\<^sub>i\<^sub>g"
+          assume h2: "\<rho> \<in> \<lbrakk> ((K\<^sub>3 \<Up> n) # (K\<^sub>2 \<Down> n @\<sharp> \<lparr>\<tau>\<^sub>v\<^sub>a\<^sub>r(K\<^sub>2, n) \<oplus> \<delta>\<tau>\<rparr>) # (K\<^sub>1 \<Up> n) # \<Gamma>), n \<turnstile> \<Psi> \<triangleright> ((K\<^sub>1 time-delayed\<sharp> by \<delta>\<tau> on K\<^sub>2 implies K\<^sub>3) # \<Phi>) \<rbrakk>\<^sub>c\<^sub>o\<^sub>n\<^sub>f\<^sub>i\<^sub>g"
           then have "\<exists>\<Gamma>\<^sub>k \<Psi>\<^sub>k \<Phi>\<^sub>k k.
-              ((((K\<^sub>3 \<Up> n) # (K\<^sub>2 \<Down> n @@ \<lparr>\<tau>\<^sub>v\<^sub>a\<^sub>r(K\<^sub>2, n) \<oplus> \<delta>\<tau>\<rparr>) # (K\<^sub>1 \<Up> n) # \<Gamma>), n \<turnstile> \<Psi> \<triangleright> ((K\<^sub>1 time-delayed2 by \<delta>\<tau> on K\<^sub>2 implies K\<^sub>3) # \<Phi>)) \<hookrightarrow>\<^bsup>k\<^esup> (\<Gamma>\<^sub>k, Suc n \<turnstile> \<Psi>\<^sub>k \<triangleright> \<Phi>\<^sub>k))
+              ((((K\<^sub>3 \<Up> n) # (K\<^sub>2 \<Down> n @\<sharp> \<lparr>\<tau>\<^sub>v\<^sub>a\<^sub>r(K\<^sub>2, n) \<oplus> \<delta>\<tau>\<rparr>) # (K\<^sub>1 \<Up> n) # \<Gamma>), n \<turnstile> \<Psi> \<triangleright> ((K\<^sub>1 time-delayed\<sharp> by \<delta>\<tau> on K\<^sub>2 implies K\<^sub>3) # \<Phi>)) \<hookrightarrow>\<^bsup>k\<^esup> (\<Gamma>\<^sub>k, Suc n \<turnstile> \<Psi>\<^sub>k \<triangleright> \<Phi>\<^sub>k))
             \<and> \<rho> \<in> \<lbrakk> \<Gamma>\<^sub>k, Suc n \<turnstile> \<Psi>\<^sub>k \<triangleright> \<Phi>\<^sub>k \<rbrakk>\<^sub>c\<^sub>o\<^sub>n\<^sub>f\<^sub>i\<^sub>g"
-            using h2 TimeDelayedBy2.prems by simp
+            using h2 TimeDelayedByTvar.prems by simp
           then show ?thesis
-            by (meson elims_part relpowp_Suc_I2 timedelayed2_e2 sporadic_add_e2)
+            by (meson elims_part relpowp_Suc_I2 timedelayed_tvar_e2 sporadic_on_tvar_e2)
         qed
-        ultimately show ?case using TimeDelayedBy2.prems(2) by (metis UnE branches more_branches)
+        ultimately show ?case using TimeDelayedByTvar.prems(2) by (metis UnE branches more_branches)
   next
     case (WeaklyPrecedes K\<^sub>1 K\<^sub>2)
       have \<open>\<lbrakk> \<Gamma>, n \<turnstile> ((K\<^sub>1 weakly precedes K\<^sub>2) # \<Psi>) \<triangleright> \<Phi> \<rbrakk>\<^sub>c\<^sub>o\<^sub>n\<^sub>f\<^sub>i\<^sub>g =
         \<lbrakk> ((\<lceil>#\<^sup>\<le> K\<^sub>2 n, #\<^sup>\<le> K\<^sub>1 n\<rceil> \<in> (\<lambda>(x, y). x \<le> y)) # \<Gamma>), n
             \<turnstile> \<Psi> \<triangleright> ((K\<^sub>1 weakly precedes K\<^sub>2) # \<Phi>) \<rbrakk>\<^sub>c\<^sub>o\<^sub>n\<^sub>f\<^sub>i\<^sub>g\<close>
-        using HeronConf_interp_stepwise_weakly_precedes_cases by simp
+        using configuration_interp_stepwise_weakly_precedes_cases by simp
       moreover have \<open>\<rho> \<in> \<lbrakk> ((\<lceil>#\<^sup>\<le> K\<^sub>2 n, #\<^sup>\<le> K\<^sub>1 n\<rceil> \<in> (\<lambda>(x, y). x \<le> y)) # \<Gamma>), n
                             \<turnstile> \<Psi> \<triangleright> ((K\<^sub>1 weakly precedes K\<^sub>2) # \<Phi>) \<rbrakk>\<^sub>c\<^sub>o\<^sub>n\<^sub>f\<^sub>i\<^sub>g
             \<Longrightarrow> (\<exists>\<Gamma>\<^sub>k \<Psi>\<^sub>k \<Phi>\<^sub>k k. ((\<Gamma>, n \<turnstile> ((K\<^sub>1 weakly precedes K\<^sub>2) # \<Psi>) \<triangleright> \<Phi>)
@@ -753,7 +753,7 @@ next
       have \<open>\<lbrakk> \<Gamma>, n \<turnstile> ((K\<^sub>1 strictly precedes K\<^sub>2) # \<Psi>) \<triangleright> \<Phi> \<rbrakk>\<^sub>c\<^sub>o\<^sub>n\<^sub>f\<^sub>i\<^sub>g =
         \<lbrakk> ((\<lceil>#\<^sup>\<le> K\<^sub>2 n, #\<^sup>< K\<^sub>1 n\<rceil> \<in> (\<lambda>(x, y). x \<le> y)) # \<Gamma>), n
           \<turnstile> \<Psi> \<triangleright> ((K\<^sub>1 strictly precedes K\<^sub>2) # \<Phi>) \<rbrakk>\<^sub>c\<^sub>o\<^sub>n\<^sub>f\<^sub>i\<^sub>g\<close>
-        using HeronConf_interp_stepwise_strictly_precedes_cases by simp
+        using configuration_interp_stepwise_strictly_precedes_cases by simp
       moreover have \<open>\<rho> \<in> \<lbrakk> ((\<lceil>#\<^sup>\<le> K\<^sub>2 n, #\<^sup>< K\<^sub>1 n\<rceil> \<in> (\<lambda>(x, y). x \<le> y)) # \<Gamma>), n
                             \<turnstile> \<Psi> \<triangleright> ((K\<^sub>1 strictly precedes K\<^sub>2) # \<Phi>) \<rbrakk>\<^sub>c\<^sub>o\<^sub>n\<^sub>f\<^sub>i\<^sub>g
             \<Longrightarrow> (\<exists>\<Gamma>\<^sub>k \<Psi>\<^sub>k \<Phi>\<^sub>k k. ((\<Gamma>, n \<turnstile> ((K\<^sub>1 strictly precedes K\<^sub>2) # \<Psi>) \<triangleright> \<Phi>)
@@ -787,7 +787,7 @@ next
       have branches: \<open>\<lbrakk> \<Gamma>, n \<turnstile> ((K\<^sub>1 kills K\<^sub>2) # \<Psi>) \<triangleright> \<Phi> \<rbrakk>\<^sub>c\<^sub>o\<^sub>n\<^sub>f\<^sub>i\<^sub>g
           = \<lbrakk> ((K\<^sub>1 \<not>\<Up> n) # \<Gamma>), n \<turnstile> \<Psi> \<triangleright> ((K\<^sub>1 kills K\<^sub>2) # \<Phi>) \<rbrakk>\<^sub>c\<^sub>o\<^sub>n\<^sub>f\<^sub>i\<^sub>g
           \<union> \<lbrakk> ((K\<^sub>1 \<Up> n) # (K\<^sub>2 \<not>\<Up> \<ge> n) # \<Gamma>), n \<turnstile> \<Psi> \<triangleright> ((K\<^sub>1 kills K\<^sub>2) # \<Phi>) \<rbrakk>\<^sub>c\<^sub>o\<^sub>n\<^sub>f\<^sub>i\<^sub>g\<close>
-        using HeronConf_interp_stepwise_kills_cases by simp
+        using configuration_interp_stepwise_kills_cases by simp
       moreover have br1: \<open>\<rho> \<in> \<lbrakk> ((K\<^sub>1 \<not>\<Up> n) # \<Gamma>), n \<turnstile> \<Psi> \<triangleright> ((K\<^sub>1 kills K\<^sub>2) # \<Phi>) \<rbrakk>\<^sub>c\<^sub>o\<^sub>n\<^sub>f\<^sub>i\<^sub>g
                 \<Longrightarrow> \<exists>\<Gamma>\<^sub>k \<Psi>\<^sub>k \<Phi>\<^sub>k k. ((\<Gamma>, n \<turnstile> ((K\<^sub>1 kills K\<^sub>2) # \<Psi>) \<triangleright> \<Phi>)
                                     \<hookrightarrow>\<^bsup>k\<^esup> (\<Gamma>\<^sub>k, Suc n \<turnstile> \<Psi>\<^sub>k \<triangleright> \<Phi>\<^sub>k))
@@ -915,7 +915,7 @@ where
   \<open>\<mu> [] = (0::nat)\<close>
 | \<open>\<mu> (\<phi> # \<Phi>) = (case \<phi> of
                       _ sporadic _ on _ \<Rightarrow> 1 + \<mu> \<Phi>
-                    | _ sporadic-add _ on _ \<Rightarrow> 1 + \<mu> \<Phi>
+                    | _ sporadic\<sharp> _ on _ \<Rightarrow> 1 + \<mu> \<Phi>
                     | _                 \<Rightarrow> 2 + \<mu> \<Phi>)\<close>
 
 fun measure_interpretation_config :: \<open>'\<tau>::linordered_field config \<Rightarrow> nat\<close> (\<open>\<mu>\<^sub>c\<^sub>o\<^sub>n\<^sub>f\<^sub>i\<^sub>g\<close>)
