src/Operational.thy
@@ -60,12 +60,12 @@ where
   to satisfy, so it disappears from the future.\<close>
   \<open>(\<Gamma>, n \<turnstile> ((K\<^sub>1 sporadic \<tau> on K\<^sub>2) # \<Psi>) \<triangleright> \<Phi>)
      \<hookrightarrow>\<^sub>e  (((K\<^sub>1 \<Up> n) # (K\<^sub>2 \<Down> n @ \<tau>) # \<Gamma>), n \<turnstile> \<Psi> \<triangleright> \<Phi>)\<close>
-| sporadic_add_e1:
-  \<open>(\<Gamma>, n \<turnstile> ((K\<^sub>1 sporadic-add \<tau>\<^sub>e\<^sub>x\<^sub>p\<^sub>r on K\<^sub>2) # \<Psi>) \<triangleright> \<Phi>)
-     \<hookrightarrow>\<^sub>e  (\<Gamma>, n \<turnstile> \<Psi> \<triangleright> ((K\<^sub>1 sporadic-add \<tau>\<^sub>e\<^sub>x\<^sub>p\<^sub>r on K\<^sub>2) # \<Phi>))\<close>
-| sporadic_add_e2:
-  \<open>(\<Gamma>, n \<turnstile> ((K\<^sub>1 sporadic-add \<tau>\<^sub>e\<^sub>x\<^sub>p\<^sub>r on K\<^sub>2) # \<Psi>) \<triangleright> \<Phi>)
-     \<hookrightarrow>\<^sub>e  (((K\<^sub>1 \<Up> n) # (K\<^sub>2 \<Down> n @@ \<tau>\<^sub>e\<^sub>x\<^sub>p\<^sub>r) # \<Gamma>), n \<turnstile> \<Psi> \<triangleright> \<Phi>)\<close>
+| sporadic_on_tvar_e1:
+  \<open>(\<Gamma>, n \<turnstile> ((K\<^sub>1 sporadic\<sharp> \<tau>\<^sub>e\<^sub>x\<^sub>p\<^sub>r on K\<^sub>2) # \<Psi>) \<triangleright> \<Phi>)
+     \<hookrightarrow>\<^sub>e  (\<Gamma>, n \<turnstile> \<Psi> \<triangleright> ((K\<^sub>1 sporadic\<sharp> \<tau>\<^sub>e\<^sub>x\<^sub>p\<^sub>r on K\<^sub>2) # \<Phi>))\<close>
+| sporadic_on_tvar_e2:
+  \<open>(\<Gamma>, n \<turnstile> ((K\<^sub>1 sporadic\<sharp> \<tau>\<^sub>e\<^sub>x\<^sub>p\<^sub>r on K\<^sub>2) # \<Psi>) \<triangleright> \<Phi>)
+     \<hookrightarrow>\<^sub>e  (((K\<^sub>1 \<Up> n) # (K\<^sub>2 \<Down> n @\<sharp> \<tau>\<^sub>e\<^sub>x\<^sub>p\<^sub>r) # \<Gamma>), n \<turnstile> \<Psi> \<triangleright> \<Phi>)\<close>
 | tagrel_e:
 \<comment> \<open>A relation between time scales has to be obeyed at every instant.\<close>
   \<open>(\<Gamma>, n \<turnstile> ((time-relation \<lfloor>K\<^sub>1, K\<^sub>2\<rfloor> \<in> R) # \<Psi>) \<triangleright> \<Phi>)
@@ -106,12 +106,12 @@ where
      \<hookrightarrow>\<^sub>e  (((K\<^sub>1 \<Up> n) # (K\<^sub>2 @ n \<oplus> \<delta>\<tau> \<Rightarrow> K\<^sub>3) # \<Gamma>), n
             \<turnstile> \<Psi> \<triangleright> ((K\<^sub>1 time-delayed by \<delta>\<tau> on K\<^sub>2 implies K\<^sub>3) # \<Phi>))\<close>
 (* Targets operational use *)
-| timedelayed2_e1:
-  \<open>(\<Gamma>, n \<turnstile> ((K\<^sub>1 time-delayed2 by \<delta>\<tau> on K\<^sub>2 implies K\<^sub>3) # \<Psi>) \<triangleright> \<Phi>)
-     \<hookrightarrow>\<^sub>e  (((K\<^sub>1 \<not>\<Up> n) # \<Gamma>), n \<turnstile> \<Psi> \<triangleright> ((K\<^sub>1 time-delayed2 by \<delta>\<tau> on K\<^sub>2 implies K\<^sub>3) # \<Phi>))\<close>
-| timedelayed2_e2:
-  \<open>(\<Gamma>, n \<turnstile> ((K\<^sub>1 time-delayed2 by \<delta>\<tau> on K\<^sub>2 implies K\<^sub>3) # \<Psi>) \<triangleright> \<Phi>)
-     \<hookrightarrow>\<^sub>e  (((K\<^sub>1 \<Up> n) # \<Gamma>), n \<turnstile> ((K\<^sub>3 sporadic-add \<lparr>\<tau>\<^sub>v\<^sub>a\<^sub>r(K\<^sub>2, n) \<oplus> \<delta>\<tau>\<rparr> on K\<^sub>2) # \<Psi>) \<triangleright> ((K\<^sub>1 time-delayed2 by \<delta>\<tau> on K\<^sub>2 implies K\<^sub>3) # \<Phi>))\<close>
+| timedelayed_tvar_e1:
+  \<open>(\<Gamma>, n \<turnstile> ((K\<^sub>1 time-delayed\<sharp> by \<delta>\<tau> on K\<^sub>2 implies K\<^sub>3) # \<Psi>) \<triangleright> \<Phi>)
+     \<hookrightarrow>\<^sub>e  (((K\<^sub>1 \<not>\<Up> n) # \<Gamma>), n \<turnstile> \<Psi> \<triangleright> ((K\<^sub>1 time-delayed\<sharp> by \<delta>\<tau> on K\<^sub>2 implies K\<^sub>3) # \<Phi>))\<close>
+| timedelayed_tvar_e2:
+  \<open>(\<Gamma>, n \<turnstile> ((K\<^sub>1 time-delayed\<sharp> by \<delta>\<tau> on K\<^sub>2 implies K\<^sub>3) # \<Psi>) \<triangleright> \<Phi>)
+     \<hookrightarrow>\<^sub>e  (((K\<^sub>1 \<Up> n) # \<Gamma>), n \<turnstile> ((K\<^sub>3 sporadic\<sharp> \<lparr>\<tau>\<^sub>v\<^sub>a\<^sub>r(K\<^sub>2, n) \<oplus> \<delta>\<tau>\<rparr> on K\<^sub>2) # \<Psi>) \<triangleright> ((K\<^sub>1 time-delayed\<sharp> by \<delta>\<tau> on K\<^sub>2 implies K\<^sub>3) # \<Phi>))\<close>
 | weakly_precedes_e:
 \<comment> \<open>A weak precedence relation has to hold at every instant.\<close>
   \<open>(\<Gamma>, n \<turnstile> ((K\<^sub>1 weakly precedes K\<^sub>2) # \<Psi>) \<triangleright> \<Phi>)
@@ -221,11 +221,13 @@ by (simp add: operational_semantics_step.simps
               operational_semantics_elim.sporadic_on_e1
               operational_semantics_elim.sporadic_on_e2)
 
-lemma Cnext_solve_sporadicon_add:
-  \<open>(\<C>\<^sub>n\<^sub>e\<^sub>x\<^sub>t (\<Gamma>, n \<turnstile> ((K\<^sub>1 sporadic-add \<tau>\<^sub>e\<^sub>x\<^sub>p\<^sub>r on K\<^sub>2) # \<Psi>) \<triangleright> \<Phi>))
-    \<supseteq> { \<Gamma>, n \<turnstile> \<Psi> \<triangleright> ((K\<^sub>1 sporadic-add \<tau>\<^sub>e\<^sub>x\<^sub>p\<^sub>r on K\<^sub>2) # \<Phi>),
-        ((K\<^sub>1 \<Up> n) # (K\<^sub>2 \<Down> n @ \<tau>) # \<Gamma>), n \<turnstile> \<Psi> \<triangleright> \<Phi> }\<close>
-  sorry
+lemma Cnext_solve_sporadicon_tvar:
+  \<open>(\<C>\<^sub>n\<^sub>e\<^sub>x\<^sub>t (\<Gamma>, n \<turnstile> ((K\<^sub>1 sporadic\<sharp> \<tau>\<^sub>e\<^sub>x\<^sub>p\<^sub>r on K\<^sub>2) # \<Psi>) \<triangleright> \<Phi>))
+    \<supseteq> { \<Gamma>, n \<turnstile> \<Psi> \<triangleright> ((K\<^sub>1 sporadic\<sharp> \<tau>\<^sub>e\<^sub>x\<^sub>p\<^sub>r on K\<^sub>2) # \<Phi>),
+        ((K\<^sub>1 \<Up> n) # (K\<^sub>2 \<Down> n @\<sharp> \<tau>\<^sub>e\<^sub>x\<^sub>p\<^sub>r) # \<Gamma>), n \<turnstile> \<Psi> \<triangleright> \<Phi> }\<close>
+by (simp add: operational_semantics_step.simps
+              operational_semantics_elim.sporadic_on_tvar_e1
+              operational_semantics_elim.sporadic_on_tvar_e2)
 
 lemma Cnext_solve_tagrel:
   \<open>(\<C>\<^sub>n\<^sub>e\<^sub>x\<^sub>t (\<Gamma>, n \<turnstile> ((time-relation \<lfloor>K\<^sub>1, K\<^sub>2\<rfloor> \<in> R) # \<Psi>) \<triangleright> \<Phi>))
@@ -257,12 +259,14 @@ by (simp add: operational_semantics_step.simps
               operational_semantics_elim.timedelayed_e1
               operational_semantics_elim.timedelayed_e2)
 
-lemma Cnext_solve_timedelayed2:
-  \<open>(\<C>\<^sub>n\<^sub>e\<^sub>x\<^sub>t (\<Gamma>, n \<turnstile> ((K\<^sub>1 time-delayed2 by \<delta>\<tau> on K\<^sub>2 implies K\<^sub>3) # \<Psi>) \<triangleright> \<Phi>))
-    \<supseteq> { ((K\<^sub>1 \<not>\<Up> n) # \<Gamma>), n \<turnstile> \<Psi> \<triangleright> ((K\<^sub>1 time-delayed2 by \<delta>\<tau> on K\<^sub>2 implies K\<^sub>3) # \<Phi>),
+lemma Cnext_solve_timedelayed_tvar:
+  \<open>(\<C>\<^sub>n\<^sub>e\<^sub>x\<^sub>t (\<Gamma>, n \<turnstile> ((K\<^sub>1 time-delayed\<sharp> by \<delta>\<tau> on K\<^sub>2 implies K\<^sub>3) # \<Psi>) \<triangleright> \<Phi>))
+    \<supseteq> { ((K\<^sub>1 \<not>\<Up> n) # \<Gamma>), n \<turnstile> \<Psi> \<triangleright> ((K\<^sub>1 time-delayed\<sharp> by \<delta>\<tau> on K\<^sub>2 implies K\<^sub>3) # \<Phi>),
         ((K\<^sub>1 \<Up> n) # \<Gamma>), n
-          \<turnstile> (K\<^sub>3 sporadic-add \<lparr>\<tau>\<^sub>v\<^sub>a\<^sub>r(K\<^sub>2, n) \<oplus> \<delta>\<tau>\<rparr> on K\<^sub>2) # \<Psi> \<triangleright> ((K\<^sub>1 time-delayed2 by \<delta>\<tau> on K\<^sub>2 implies K\<^sub>3) # \<Phi>) }\<close>
-  sorry
+          \<turnstile> (K\<^sub>3 sporadic\<sharp> \<lparr>\<tau>\<^sub>v\<^sub>a\<^sub>r(K\<^sub>2, n) \<oplus> \<delta>\<tau>\<rparr> on K\<^sub>2) # \<Psi> \<triangleright> ((K\<^sub>1 time-delayed\<sharp> by \<delta>\<tau> on K\<^sub>2 implies K\<^sub>3) # \<Phi>) }\<close>
+by (simp add: operational_semantics_step.simps
+              operational_semantics_elim.timedelayed_tvar_e1
+              operational_semantics_elim.timedelayed_tvar_e2)
 
 lemma Cnext_solve_weakly_precedes:
   \<open>(\<C>\<^sub>n\<^sub>e\<^sub>x\<^sub>t (\<Gamma>, n \<turnstile> ((K\<^sub>1 weakly precedes K\<^sub>2) # \<Psi>) \<triangleright> \<Phi>))
