src/SymbolicPrimitive.thy
@@ -36,8 +36,8 @@ datatype '\<tau> constr =
 \<comment> \<open>@{term \<open>c \<Down> n @ \<tau>\<close>} constrains clock @{term \<open>c\<close>} to have time @{term \<open>\<tau>\<close>}
     at instant @{term \<open>n\<close>} of the run.\<close>
   Timestamp     \<open>clock\<close>   \<open>instant_index\<close> \<open>'\<tau> tag_const\<close>         (\<open>_ \<Down> _ @ _\<close>)
-(* TODO: comments *)
-| Timestamp2    \<open>clock\<close>   \<open>instant_index\<close> \<open>'\<tau> tag_expr\<close>          (\<open>_ \<Down> _ @@ _\<close>)
+(* TODO: text *)
+| TimestampTvar    \<open>clock\<close>   \<open>instant_index\<close> \<open>'\<tau> tag_expr\<close>          (\<open>_ \<Down> _ @\<sharp> _\<close>)
 \<comment> \<open>@{term \<open>m @ n \<oplus> \<delta>t \<Rightarrow> s\<close>} constrains clock @{term \<open>s\<close>} to tick at the
     first instant at which the time on @{term \<open>m\<close>} has increased by @{term \<open>\<delta>t\<close>}
     from the value it had at instant @{term \<open>n\<close>} of the run.\<close>
@@ -56,7 +56,7 @@ datatype '\<tau> constr =
 | NotTicksFrom  \<open>clock\<close>   \<open>instant_index\<close>                        (\<open>_ \<not>\<Up> \<ge> _\<close>)
 \<comment> \<open>@{term \<open>\<lfloor>\<tau>\<^sub>1, \<tau>\<^sub>2\<rfloor> \<in> R\<close>} constrains tag variables @{term \<open>\<tau>\<^sub>1\<close>} and  @{term \<open>\<tau>\<^sub>2\<close>} 
     to be in relation @{term \<open>R\<close>}.\<close>
-| TagArith      \<open>tag_val\<close> \<open>tag_val\<close> \<open>('\<tau> tag_const \<times> '\<tau> tag_const) \<Rightarrow> bool\<close> (\<open>\<lfloor>_, _\<rfloor> \<in> _\<close>)
+| TagArith      \<open>tag_var\<close> \<open>tag_var\<close> \<open>('\<tau> tag_const \<times> '\<tau> tag_const) \<Rightarrow> bool\<close> (\<open>\<lfloor>_, _\<rfloor> \<in> _\<close>)
 \<comment> \<open>@{term \<open>\<lceil>k\<^sub>1, k\<^sub>2\<rceil> \<in> R\<close>} constrains counter expressions @{term \<open>k\<^sub>1\<close>} and  @{term \<open>k\<^sub>2\<close>} 
     to be in relation @{term \<open>R\<close>}.\<close>
 | TickCntArith  \<open>cnt_expr\<close> \<open>cnt_expr\<close> \<open>(nat \<times> nat) \<Rightarrow> bool\<close>      (\<open>\<lceil>_, _\<rceil> \<in> _\<close>)
@@ -104,7 +104,7 @@ where
 | \<open>\<lbrakk> K \<not>\<Up> < n \<rbrakk>\<^sub>p\<^sub>r\<^sub>i\<^sub>m   = {\<rho>. \<forall>i < n. \<not> ticks ((Rep_run \<rho>) i K)}\<close>
 | \<open>\<lbrakk> K \<not>\<Up> \<ge> n \<rbrakk>\<^sub>p\<^sub>r\<^sub>i\<^sub>m   = {\<rho>. \<forall>i \<ge> n. \<not> ticks ((Rep_run \<rho>) i K) }\<close>
 | \<open>\<lbrakk> K \<Down> n @ \<tau> \<rbrakk>\<^sub>p\<^sub>r\<^sub>i\<^sub>m = {\<rho>. time ((Rep_run \<rho>) n K) = \<tau> }\<close>
-| \<open>\<lbrakk> K \<Down> n @@ \<lparr>\<tau>\<^sub>v\<^sub>a\<^sub>r(K', n') \<oplus> \<delta>\<tau>\<rparr> \<rbrakk>\<^sub>p\<^sub>r\<^sub>i\<^sub>m = {\<rho>. time ((Rep_run \<rho>) n K) = time ((Rep_run \<rho>) n' K') + \<delta>\<tau> }\<close>
+| \<open>\<lbrakk> K \<Down> n @\<sharp> \<lparr>\<tau>\<^sub>v\<^sub>a\<^sub>r(K', n') \<oplus> \<delta>\<tau>\<rparr> \<rbrakk>\<^sub>p\<^sub>r\<^sub>i\<^sub>m = {\<rho>. time ((Rep_run \<rho>) n K) = time ((Rep_run \<rho>) n' K') + \<delta>\<tau> }\<close>
 | \<open>\<lbrakk> \<lfloor>\<tau>\<^sub>v\<^sub>a\<^sub>r(K\<^sub>1, n\<^sub>1), \<tau>\<^sub>v\<^sub>a\<^sub>r(K\<^sub>2, n\<^sub>2)\<rfloor> \<in> R \<rbrakk>\<^sub>p\<^sub>r\<^sub>i\<^sub>m =
     { \<rho>. R (time ((Rep_run \<rho>) n\<^sub>1 K\<^sub>1), time ((Rep_run \<rho>) n\<^sub>2 K\<^sub>2)) }\<close>
 | \<open>\<lbrakk> \<lceil>e\<^sub>1, e\<^sub>2\<rceil> \<in> R \<rbrakk>\<^sub>p\<^sub>r\<^sub>i\<^sub>m = { \<rho>. R (\<lbrakk> \<rho> \<turnstile> e\<^sub>1 \<rbrakk>\<^sub>c\<^sub>n\<^sub>t\<^sub>e\<^sub>x\<^sub>p\<^sub>r, \<lbrakk> \<rho> \<turnstile> e\<^sub>2 \<rbrakk>\<^sub>c\<^sub>n\<^sub>t\<^sub>e\<^sub>x\<^sub>p\<^sub>r) }\<close>
